updated vcfloat FPBench tests

FPBench/vcfloat_tests.v
@@ -1,527 +1,839 @@
-From vcfloat Require Import Automate FPLang FPLangOpt RAux Rounding Reify Float_notations.
+From vcfloat Require Import Automate Prune FPLang FPLangOpt RAux Rounding Reify Float_notations.
 Require Import IntervalFlocq3.Tactic.
 Import Binary List ListNotations.
+Set Bullet Behavior "Strict Subproofs".
 Section WITHNANS.
 Context {NANS:Nans}.
+Open Scope R_scope.
 
-Definition ex0_bmap_list := [Build_varinfo Tdouble 1%positive (-10) (10);Build_varinfo Tdouble 2%positive (-10) (10);Build_varinfo Tdouble 3%positive (-10) (10);Build_varinfo Tdouble 4%positive (-10) (10);Build_varinfo Tdouble 5%positive (-10) (10);Build_varinfo Tdouble 6%positive (-10) (10);Build_varinfo Tdouble 7%positive (-10) (10);Build_varinfo Tdouble 8%positive (-10) (10);Build_varinfo Tdouble 9%positive (-10) (10)].
+Definition matrixdeterminant_bmap_list := [Build_varinfo Tdouble 1%positive (-10) (10);Build_varinfo Tdouble 2%positive (-10) (10);Build_varinfo Tdouble 3%positive (-10) (10);Build_varinfo Tdouble 4%positive (-10) (10);Build_varinfo Tdouble 5%positive (-10) (10);Build_varinfo Tdouble 6%positive (-10) (10);Build_varinfo Tdouble 7%positive (-10) (10);Build_varinfo Tdouble 8%positive (-10) (10);Build_varinfo Tdouble 9%positive (-10) (10)].
 
-Definition ex0_bmap :=
- ltac:(let z := compute_PTree (boundsmap_of_list ex0_bmap_list) in exact z).
+Definition matrixdeterminant_bmap :=
+ ltac:(let z := compute_PTree (boundsmap_of_list matrixdeterminant_bmap_list) in exact z).
 
-Definition ex0_vmap_list (a : ftype Tdouble) (b : ftype Tdouble) (c : ftype Tdouble) (d : ftype Tdouble) (e : ftype Tdouble) (f : ftype Tdouble) (g : ftype Tdouble) (h : ftype Tdouble) (i : ftype Tdouble) := [(1%positive, existT ftype Tdouble a);(2%positive, existT ftype Tdouble b);(3%positive, existT ftype Tdouble c);(4%positive, existT ftype Tdouble d);(5%positive, existT ftype Tdouble e);(6%positive, existT ftype Tdouble f);(7%positive, existT ftype Tdouble g);(8%positive, existT ftype Tdouble h);(9%positive, existT ftype Tdouble i)].
+Definition matrixdeterminant (a : ftype Tdouble) (b : ftype Tdouble) (c : ftype Tdouble) (d : ftype Tdouble) (e : ftype Tdouble) (f : ftype Tdouble) (g : ftype Tdouble) (h : ftype Tdouble) (i : ftype Tdouble) := 
+  cast Tdouble _ ((((((a * e)%F64 * i)%F64 + ((b * f)%F64 * g)%F64)%F64 + ((c * d)%F64 * h)%F64)%F64 - ((((c * e)%F64 * g)%F64 + ((b * d)%F64 * i)%F64)%F64 + ((a * f)%F64 * h)%F64)%F64)%F64).
 
-Definition ex0_vmap (a : ftype Tdouble) (b : ftype Tdouble) (c : ftype Tdouble) (d : ftype Tdouble) (e : ftype Tdouble) (f : ftype Tdouble) (g : ftype Tdouble) (h : ftype Tdouble) (i : ftype Tdouble) :=
- ltac:(let z := compute_PTree (valmap_of_list (ex0_vmap_list a  b  c  d  e  f  g  h  i )) in exact z).
+Definition matrixdeterminant_expr := 
+ ltac:(let e' :=  HO_reify_float_expr constr:([1%positive;2%positive;3%positive;4%positive;5%positive;6%positive;7%positive;8%positive;9%positive]) matrixdeterminant in exact e').
 
-Definition ex0 (a : ftype Tdouble) (b : ftype Tdouble) (c : ftype Tdouble) (d : ftype Tdouble) (e : ftype Tdouble) (f : ftype Tdouble) 
-(g : ftype Tdouble) (h : ftype Tdouble) (i : ftype Tdouble) := 
-  cast Tdouble _ ((cast Tdouble _ ((cast Tdouble _ ((cast Tdouble _ ((cast Tdouble _ ((cast Tdouble _ (a) * cast Tdouble _ (e))%F64) * cast Tdouble _ (i))%F64) + cast Tdouble _ ((cast Tdouble _ ((cast Tdouble _ (b) * cast Tdouble _ (f))%F64) * cast Tdouble _ (g))%F64))%F64) + cast Tdouble _ ((cast Tdouble _ ((cast Tdouble _ (c) * cast Tdouble _ (d))%F64) * cast Tdouble _ (h))%F64))%F64) - cast Tdouble _ ((cast Tdouble _ ((cast Tdouble _ ((cast Tdouble _ ((cast Tdouble _ (c) * cast Tdouble _ (e))%F64) * cast Tdouble _ (g))%F64) + cast Tdouble _ ((cast Tdouble _ ((cast Tdouble _ (b) * cast Tdouble _ (d))%F64) * cast Tdouble _ (i))%F64))%F64) + cast Tdouble _ ((cast Tdouble _ ((cast Tdouble _ (a) * cast Tdouble _ (f))%F64) * cast Tdouble _ (h))%F64))%F64))%F64).
+Lemma matrixdeterminant_bound:
+	find_and_prove_roundoff_bound matrixdeterminant_bmap matrixdeterminant_expr.
+Proof.
+eexists. intro. prove_roundoff_bound.
+ -
+time "prove_rndval" prove_rndval; time "interval" interval.
+-
+time "prove_roundoff_bound2" prove_roundoff_bound2;
+time "prune_terms" (prune_terms (cutoff 30)).
+time "do_interval" do_interval.
+Defined.
 
-Definition ex0_expr := 
- ltac:(let e' :=  HO_reify_float_expr constr:([1%positive;2%positive;3%positive;4%positive;5%positive;6%positive;7%positive;8%positive;9%positive]) ex0 in exact e').
+Definition matrixdeterminant_bound_val := Eval simpl in (proj1_sig matrixdeterminant_bound).
+Print matrixdeterminant_bound_val.
 
-Definition ex1_bmap_list := [Build_varinfo Tdouble 1%positive (-10) (10);Build_varinfo Tdouble 2%positive (-10) (10);Build_varinfo Tdouble 3%positive (-10) (10);Build_varinfo Tdouble 4%positive (-10) (10);Build_varinfo Tdouble 5%positive (-10) (10);Build_varinfo Tdouble 6%positive (-10) (10);Build_varinfo Tdouble 7%positive (-10) (10);Build_varinfo Tdouble 8%positive (-10) (10);Build_varinfo Tdouble 9%positive (-10) (10)].
+Definition matrixdeterminant2_bmap_list := [Build_varinfo Tdouble 1%positive (-10) (10);Build_varinfo Tdouble 2%positive (-10) (10);Build_varinfo Tdouble 3%positive (-10) (10);Build_varinfo Tdouble 4%positive (-10) (10);Build_varinfo Tdouble 5%positive (-10) (10);Build_varinfo Tdouble 6%positive (-10) (10);Build_varinfo Tdouble 7%positive (-10) (10);Build_varinfo Tdouble 8%positive (-10) (10);Build_varinfo Tdouble 9%positive (-10) (10)].
 
-Definition ex1_bmap :=
- ltac:(let z := compute_PTree (boundsmap_of_list ex1_bmap_list) in exact z).
+Definition matrixdeterminant2_bmap :=
+ ltac:(let z := compute_PTree (boundsmap_of_list matrixdeterminant2_bmap_list) in exact z).
 
-Definition ex1_vmap_list (a : ftype Tdouble) (b : ftype Tdouble) (c : ftype Tdouble) (d : ftype Tdouble) (e : ftype Tdouble) (f : ftype Tdouble) (g : ftype Tdouble) (h : ftype Tdouble) (i : ftype Tdouble) := [(1%positive, existT ftype Tdouble a);(2%positive, existT ftype Tdouble b);(3%positive, existT ftype Tdouble c);(4%positive, existT ftype Tdouble d);(5%positive, existT ftype Tdouble e);(6%positive, existT ftype Tdouble f);(7%positive, existT ftype Tdouble g);(8%positive, existT ftype Tdouble h);(9%positive, existT ftype Tdouble i)].
+Definition matrixdeterminant2 (a : ftype Tdouble) (b : ftype Tdouble) (c : ftype Tdouble) (d : ftype Tdouble) (e : ftype Tdouble) (f : ftype Tdouble) (g : ftype Tdouble) (h : ftype Tdouble) (i : ftype Tdouble) := 
+  cast Tdouble _ ((((a * (e * i)%F64)%F64 + ((g * (b * f)%F64)%F64 + (c * (d * h)%F64)%F64)%F64)%F64 - ((e * (c * g)%F64)%F64 + ((i * (b * d)%F64)%F64 + (a * (f * h)%F64)%F64)%F64)%F64)%F64).
 
-Definition ex1_vmap (a : ftype Tdouble) (b : ftype Tdouble) (c : ftype Tdouble) (d : ftype Tdouble) (e : ftype Tdouble) (f : ftype Tdouble) (g : ftype Tdouble) (h : ftype Tdouble) (i : ftype Tdouble) :=
- ltac:(let z := compute_PTree (valmap_of_list (ex1_vmap_list a  b  c  d  e  f  g  h  i )) in exact z).
+Definition matrixdeterminant2_expr := 
+ ltac:(let e' :=  HO_reify_float_expr constr:([1%positive;2%positive;3%positive;4%positive;5%positive;6%positive;7%positive;8%positive;9%positive]) matrixdeterminant2 in exact e').
 
-Definition ex1 (a : ftype Tdouble) (b : ftype Tdouble) (c : ftype Tdouble) (d : ftype Tdouble) (e : ftype Tdouble) (f : ftype Tdouble) (g : ftype Tdouble) (h : ftype Tdouble) (i : ftype Tdouble) := 
-  cast Tdouble _ ((cast Tdouble _ ((cast Tdouble _ ((cast Tdouble _ (a) * cast Tdouble _ ((cast Tdouble _ (e) * cast Tdouble _ (i))%F64))%F64) + cast Tdouble _ ((cast Tdouble _ ((cast Tdouble _ (g) * cast Tdouble _ ((cast Tdouble _ (b) * cast Tdouble _ (f))%F64))%F64) + cast Tdouble _ ((cast Tdouble _ (c) * cast Tdouble _ ((cast Tdouble _ (d) * cast Tdouble _ (h))%F64))%F64))%F64))%F64) - cast Tdouble _ ((cast Tdouble _ ((cast Tdouble _ (e) * cast Tdouble _ ((cast Tdouble _ (c) * cast Tdouble _ (g))%F64))%F64) + cast Tdouble _ ((cast Tdouble _ ((cast Tdouble _ (i) * cast Tdouble _ ((cast Tdouble _ (b) * cast Tdouble _ (d))%F64))%F64) + cast Tdouble _ ((cast Tdouble _ (a) * cast Tdouble _ ((cast Tdouble _ (f) * cast Tdouble _ (h))%F64))%F64))%F64))%F64))%F64).
+Lemma matrixdeterminant2_bound:
+	find_and_prove_roundoff_bound matrixdeterminant2_bmap matrixdeterminant2_expr.
+Proof.
+eexists. intro. prove_roundoff_bound.
+ -
+time "prove_rndval" prove_rndval; time "interval" interval.
+-
+time "prove_roundoff_bound2" prove_roundoff_bound2;
+time "prune_terms" (prune_terms (cutoff 30)).
+time "do_interval" do_interval.
+Defined.
 
-Definition ex1_expr := 
- ltac:(let e' :=  HO_reify_float_expr constr:([1%positive;2%positive;3%positive;4%positive;5%positive;6%positive;7%positive;8%positive;9%positive]) ex1 in exact e').
+Definition matrixdeterminant2_bound_val := Eval simpl in (proj1_sig matrixdeterminant2_bound).
+Print matrixdeterminant2_bound_val.
 
-Definition ex2_bmap_list := [Build_varinfo Tsingle 1%positive (1) (999)].
+Definition intro_45_example_45_mixed_bmap_list := [Build_varinfo Tsingle 1%positive (1) (999)].
 
-Definition ex2_bmap :=
- ltac:(let z := compute_PTree (boundsmap_of_list ex2_bmap_list) in exact z).
+Definition intro_45_example_45_mixed_bmap :=
+ ltac:(let z := compute_PTree (boundsmap_of_list intro_45_example_45_mixed_bmap_list) in exact z).
 
-Definition ex2_vmap_list (t : ftype Tsingle) := [(1%positive, existT ftype Tsingle t)].
-
-Definition ex2_vmap (t : ftype Tsingle) :=
- ltac:(let z := compute_PTree (valmap_of_list (ex2_vmap_list t )) in exact z).
-
-Definition ex2 (t : ftype Tsingle) := 
-  cast Tsingle _ (let t_1 := let t1_2 := (cast Tsingle _ (t) + cast Tsingle _ (cast Tsingle Tsingle (1)%F32))%F32 in
+Definition intro_45_example_45_mixed (t : ftype Tsingle) := 
+  cast Tsingle _ (let t_1 := let t1_2 := (t + (1)%F32)%F32 in
       (cast Tdouble _ (t) / cast Tdouble _ (t1_2))%F64 in
   cast Tsingle _ (t_1)).
 
-Definition ex2_expr := 
- ltac:(let e' :=  HO_reify_float_expr constr:([1%positive]) ex2 in exact e').
-
-Definition ex3_bmap_list := [Build_varinfo Tdouble 1%positive (4) (63504e-4);Build_varinfo Tdouble 2%positive (4) (63504e-4);Build_varinfo Tdouble 3%positive (4) (63504e-4);Build_varinfo Tdouble 4%positive (4) (63504e-4);Build_varinfo Tdouble 5%positive (4) (63504e-4);Build_varinfo Tdouble 6%positive (4) (63504e-4)].
-
-Definition ex3_bmap :=
- ltac:(let z := compute_PTree (boundsmap_of_list ex3_bmap_list) in exact z).
-
-Definition ex3_vmap_list (x1 : ftype Tdouble) (x2 : ftype Tdouble) (x3 : ftype Tdouble) (x4 : ftype Tdouble) (x5 : ftype Tdouble) (x6 : ftype Tdouble) := [(1%positive, existT ftype Tdouble x1);(2%positive, existT ftype Tdouble x2);(3%positive, existT ftype Tdouble x3);(4%positive, existT ftype Tdouble x4);(5%positive, existT ftype Tdouble x5);(6%positive, existT ftype Tdouble x6)].
-
-Definition ex3_vmap (x1 : ftype Tdouble) (x2 : ftype Tdouble) (x3 : ftype Tdouble) (x4 : ftype Tdouble) (x5 : ftype Tdouble) (x6 : ftype Tdouble) :=
- ltac:(let z := compute_PTree (valmap_of_list (ex3_vmap_list x1  x2  x3  x4  x5  x6 )) in exact z).
-
-Definition ex3 (x1 : ftype Tdouble) (x2 : ftype Tdouble) (x3 : ftype Tdouble) (x4 : ftype Tdouble) (x5 : ftype Tdouble) (x6 : ftype Tdouble) := 
-  cast Tdouble _ ((cast Tdouble _ ((cast Tdouble _ ((cast Tdouble _ ((cast Tdouble _ ((cast Tdouble _ ((cast Tdouble _ (-x2) * cast Tdouble _ (x3))%F64) - cast Tdouble _ ((cast Tdouble _ (x1) * cast Tdouble _ (x4))%F64))%F64) + cast Tdouble _ ((cast Tdouble _ (x2) * cast Tdouble _ (x5))%F64))%F64) + cast Tdouble _ ((cast Tdouble _ (x3) * cast Tdouble _ (x6))%F64))%F64) - cast Tdouble _ ((cast Tdouble _ (x5) * cast Tdouble _ (x6))%F64))%F64) + cast Tdouble _ ((cast Tdouble _ (x1) * cast Tdouble _ ((cast Tdouble _ ((cast Tdouble _ ((cast Tdouble _ ((cast Tdouble _ ((cast Tdouble _ (-x1) + cast Tdouble _ (x2))%F64) + cast Tdouble _ (x3))%F64) - cast Tdouble _ (x4))%F64) + cast Tdouble _ (x5))%F64) + cast Tdouble _ (x6))%F64))%F64))%F64).
-
-Definition ex3_expr := 
- ltac:(let e' :=  HO_reify_float_expr constr:([1%positive;2%positive;3%positive;4%positive;5%positive;6%positive]) ex3 in exact e').
-
-Definition ex4_bmap_list := [Build_varinfo Tdouble 1%positive (4) (63504e-4);Build_varinfo Tdouble 2%positive (4) (63504e-4);Build_varinfo Tdouble 3%positive (4) (63504e-4);Build_varinfo Tdouble 4%positive (4) (63504e-4);Build_varinfo Tdouble 5%positive (4) (63504e-4);Build_varinfo Tdouble 6%positive (4) (63504e-4)].
-
-Definition ex4_bmap :=
- ltac:(let z := compute_PTree (boundsmap_of_list ex4_bmap_list) in exact z).
-
-Definition ex4_vmap_list (x1 : ftype Tdouble) (x2 : ftype Tdouble) (x3 : ftype Tdouble) (x4 : ftype Tdouble) (x5 : ftype Tdouble) (x6 : ftype Tdouble) := [(1%positive, existT ftype Tdouble x1);(2%positive, existT ftype Tdouble x2);(3%positive, existT ftype Tdouble x3);(4%positive, existT ftype Tdouble x4);(5%positive, existT ftype Tdouble x5);(6%positive, existT ftype Tdouble x6)].
-
-Definition ex4_vmap (x1 : ftype Tdouble) (x2 : ftype Tdouble) (x3 : ftype Tdouble) (x4 : ftype Tdouble) (x5 : ftype Tdouble) (x6 : ftype Tdouble) :=
- ltac:(let z := compute_PTree (valmap_of_list (ex4_vmap_list x1  x2  x3  x4  x5  x6 )) in exact z).
-
-Definition ex4 (x1 : ftype Tdouble) (x2 : ftype Tdouble) (x3 : ftype Tdouble) (x4 : ftype Tdouble) (x5 : ftype Tdouble) (x6 : ftype Tdouble) := 
-  cast Tdouble _ ((cast Tdouble _ ((cast Tdouble _ ((cast Tdouble _ ((cast Tdouble _ ((cast Tdouble _ ((cast Tdouble _ ((cast Tdouble _ ((cast Tdouble _ (x1) * cast Tdouble _ (x4))%F64) * cast Tdouble _ ((cast Tdouble _ ((cast Tdouble _ ((cast Tdouble _ ((cast Tdouble _ ((cast Tdouble _ (-x1) + cast Tdouble _ (x2))%F64) + cast Tdouble _ (x3))%F64) - cast Tdouble _ (x4))%F64) + cast Tdouble _ (x5))%F64) + cast Tdouble _ (x6))%F64))%F64) + cast Tdouble _ ((cast Tdouble _ ((cast Tdouble _ (x2) * cast Tdouble _ (x5))%F64) * cast Tdouble _ ((cast Tdouble _ ((cast Tdouble _ ((cast Tdouble _ ((cast Tdouble _ ((cast Tdouble _ (x1) - cast Tdouble _ (x2))%F64) + cast Tdouble _ (x3))%F64) + cast Tdouble _ (x4))%F64) - cast Tdouble _ (x5))%F64) + cast Tdouble _ (x6))%F64))%F64))%F64) + cast Tdouble _ ((cast Tdouble _ ((cast Tdouble _ (x3) * cast Tdouble _ (x6))%F64) * cast Tdouble _ ((cast Tdouble _ ((cast Tdouble _ ((cast Tdouble _ ((cast Tdouble _ ((cast Tdouble _ (x1) + cast Tdouble _ (x2))%F64) - cast Tdouble _ (x3))%F64) + cast Tdouble _ (x4))%F64) + cast Tdouble _ (x5))%F64) - cast Tdouble _ (x6))%F64))%F64))%F64) + cast Tdouble _ ((cast Tdouble _ ((cast Tdouble _ (-x2) * cast Tdouble _ (x3))%F64) * cast Tdouble _ (x4))%F64))%F64) + cast Tdouble _ ((cast Tdouble _ ((cast Tdouble _ (-x1) * cast Tdouble _ (x3))%F64) * cast Tdouble _ (x5))%F64))%F64) + cast Tdouble _ ((cast Tdouble _ ((cast Tdouble _ (-x1) * cast Tdouble _ (x2))%F64) * cast Tdouble _ (x6))%F64))%F64) + cast Tdouble _ ((cast Tdouble _ ((cast Tdouble _ (-x4) * cast Tdouble _ (x5))%F64) * cast Tdouble _ (x6))%F64))%F64).
-
-Definition ex4_expr := 
- ltac:(let e' :=  HO_reify_float_expr constr:([1%positive;2%positive;3%positive;4%positive;5%positive;6%positive]) ex4 in exact e').
-
-Definition ex5_bmap_list := [Build_varinfo Tsingle 1%positive (1) (4);Build_varinfo Tsingle 2%positive (1) (4)].
-
-Definition ex5_bmap :=
- ltac:(let z := compute_PTree (boundsmap_of_list ex5_bmap_list) in exact z).
-
-Definition ex5_vmap_list (x : ftype Tsingle) (y : ftype Tsingle) := [(1%positive, existT ftype Tsingle x);(2%positive, existT ftype Tsingle y)].
-
-Definition ex5_vmap (x : ftype Tsingle) (y : ftype Tsingle) :=
- ltac:(let z := compute_PTree (valmap_of_list (ex5_vmap_list x  y )) in exact z).
-
-Definition ex5 (x : ftype Tsingle) (y : ftype Tsingle) := 
-  cast Tsingle _ ((cast Tsingle _ (x) / cast Tsingle _ ((cast Tsingle _ (x) + cast Tsingle _ (y))%F32))%F32).
-
-Definition ex5_expr := 
- ltac:(let e' :=  HO_reify_float_expr constr:([1%positive;2%positive]) ex5 in exact e').
-
-Definition ex6_bmap_list := [Build_varinfo Tdouble 1%positive (1) (2);Build_varinfo Tdouble 2%positive (1) (2);Build_varinfo Tdouble 3%positive (1) (2)].
-
-Definition ex6_bmap :=
- ltac:(let z := compute_PTree (boundsmap_of_list ex6_bmap_list) in exact z).
-
-Definition ex6_vmap_list (x0 : ftype Tdouble) (x1 : ftype Tdouble) (x2 : ftype Tdouble) := [(1%positive, existT ftype Tdouble x0);(2%positive, existT ftype Tdouble x1);(3%positive, existT ftype Tdouble x2)].
-
-Definition ex6_vmap (x0 : ftype Tdouble) (x1 : ftype Tdouble) (x2 : ftype Tdouble) :=
- ltac:(let z := compute_PTree (valmap_of_list (ex6_vmap_list x0  x1  x2 )) in exact z).
-
-Definition ex6 (x0 : ftype Tdouble) (x1 : ftype Tdouble) (x2 : ftype Tdouble) := 
-  cast Tdouble _ (let p0 := (cast Tdouble _ ((cast Tdouble _ (x0) + cast Tdouble _ (x1))%F64) - cast Tdouble _ (x2))%F64 in
-  let p1 := (cast Tdouble _ ((cast Tdouble _ (x1) + cast Tdouble _ (x2))%F64) - cast Tdouble _ (x0))%F64 in
-  let p2 := (cast Tdouble _ ((cast Tdouble _ (x2) + cast Tdouble _ (x0))%F64) - cast Tdouble _ (x1))%F64 in
-  (cast Tdouble _ ((cast Tdouble _ (p0) + cast Tdouble _ (p1))%F64) + cast Tdouble _ (p2))%F64).
-
-Definition ex6_expr := 
- ltac:(let e' :=  HO_reify_float_expr constr:([1%positive;2%positive;3%positive]) ex6 in exact e').
-
-Definition ex7_bmap_list := [Build_varinfo Tdouble 1%positive (0) (999)].
-
-Definition ex7_bmap :=
- ltac:(let z := compute_PTree (boundsmap_of_list ex7_bmap_list) in exact z).
-
-Definition ex7_vmap_list (z : ftype Tdouble) := [(1%positive, existT ftype Tdouble z)].
-
-Definition ex7_vmap (z : ftype Tdouble) :=
- ltac:(let z := compute_PTree (valmap_of_list (ex7_vmap_list z )) in exact z).
-
-Definition ex7 (z : ftype Tdouble) := 
-  cast Tdouble _ ((cast Tdouble _ (z) / cast Tdouble _ ((cast Tdouble _ (z) + cast Tdouble _ (cast Tdouble Tdouble (1)%F64))%F64))%F64).
-
-Definition ex7_expr := 
- ltac:(let e' :=  HO_reify_float_expr constr:([1%positive]) ex7 in exact e').
-
-Definition ex8_bmap_list := [Build_varinfo Tdouble 1%positive (1001e-3) (2);Build_varinfo Tdouble 2%positive (1001e-3) (2)].
-
-Definition ex8_bmap :=
- ltac:(let z := compute_PTree (boundsmap_of_list ex8_bmap_list) in exact z).
-
-Definition ex8_vmap_list (x : ftype Tdouble) (y : ftype Tdouble) := [(1%positive, existT ftype Tdouble x);(2%positive, existT ftype Tdouble y)].
-
-Definition ex8_vmap (x : ftype Tdouble) (y : ftype Tdouble) :=
- ltac:(let z := compute_PTree (valmap_of_list (ex8_vmap_list x  y )) in exact z).
-
-Definition ex8 (x : ftype Tdouble) (y : ftype Tdouble) := 
-  cast Tdouble _ (let t := (cast Tdouble _ (x) * cast Tdouble _ (y))%F64 in
-  (cast Tdouble _ ((cast Tdouble _ (t) - cast Tdouble _ (cast Tdouble Tdouble (1)%F64))%F64) / cast Tdouble _ ((cast Tdouble _ ((cast Tdouble _ (t) * cast Tdouble _ (t))%F64) - cast Tdouble _ (cast Tdouble Tdouble (1)%F64))%F64))%F64).
-
-Definition ex8_expr := 
- ltac:(let e' :=  HO_reify_float_expr constr:([1%positive;2%positive]) ex8 in exact e').
-
-Definition ex9_bmap_list := [Build_varinfo Tdouble 1%positive (-5) (5);Build_varinfo Tdouble 2%positive (-5) (5)].
-
-Definition ex9_bmap :=
- ltac:(let z := compute_PTree (boundsmap_of_list ex9_bmap_list) in exact z).
-
-Definition ex9_vmap_list (x1 : ftype Tdouble) (x2 : ftype Tdouble) := [(1%positive, existT ftype Tdouble x1);(2%positive, existT ftype Tdouble x2)].
-
-Definition ex9_vmap (x1 : ftype Tdouble) (x2 : ftype Tdouble) :=
- ltac:(let z := compute_PTree (valmap_of_list (ex9_vmap_list x1  x2 )) in exact z).
-
-Definition ex9 (x1 : ftype Tdouble) (x2 : ftype Tdouble) := 
-  cast Tdouble _ (let a := (cast Tdouble _ ((cast Tdouble _ ((cast Tdouble _ (x1) * cast Tdouble _ (x1))%F64) + cast Tdouble _ (x2))%F64) - cast Tdouble _ (cast Tdouble Tdouble (11)%F64))%F64 in
-  let b := (cast Tdouble _ ((cast Tdouble _ (x1) + cast Tdouble _ ((cast Tdouble _ (x2) * cast Tdouble _ (x2))%F64))%F64) - cast Tdouble _ (cast Tdouble Tdouble (7)%F64))%F64 in
-  (cast Tdouble _ ((cast Tdouble _ (a) * cast Tdouble _ (a))%F64) + cast Tdouble _ ((cast Tdouble _ (b) * cast Tdouble _ (b))%F64))%F64).
-
-Definition ex9_expr := 
- ltac:(let e' :=  HO_reify_float_expr constr:([1%positive;2%positive]) ex9 in exact e').
-
-Definition ex10_bmap_list := [Build_varinfo Tdouble 1%positive (4) (636e-2);Build_varinfo Tdouble 2%positive (4) (636e-2);Build_varinfo Tdouble 3%positive (4) (636e-2);Build_varinfo Tdouble 4%positive (4) (636e-2);Build_varinfo Tdouble 5%positive (4) (636e-2);Build_varinfo Tdouble 6%positive (4) (636e-2)].
-
-Definition ex10_bmap :=
- ltac:(let z := compute_PTree (boundsmap_of_list ex10_bmap_list) in exact z).
-
-Definition ex10_vmap_list (x1 : ftype Tdouble) (x2 : ftype Tdouble) (x3 : ftype Tdouble) (x4 : ftype Tdouble) (x5 : ftype Tdouble) (x6 : ftype Tdouble) := [(1%positive, existT ftype Tdouble x1);(2%positive, existT ftype Tdouble x2);(3%positive, existT ftype Tdouble x3);(4%positive, existT ftype Tdouble x4);(5%positive, existT ftype Tdouble x5);(6%positive, existT ftype Tdouble x6)].
-
-Definition ex10_vmap (x1 : ftype Tdouble) (x2 : ftype Tdouble) (x3 : ftype Tdouble) (x4 : ftype Tdouble) (x5 : ftype Tdouble) (x6 : ftype Tdouble) :=
- ltac:(let z := compute_PTree (valmap_of_list (ex10_vmap_list x1  x2  x3  x4  x5  x6 )) in exact z).
-
-Definition ex10 (x1 : ftype Tdouble) (x2 : ftype Tdouble) (x3 : ftype Tdouble) (x4 : ftype Tdouble) (x5 : ftype Tdouble) (x6 : ftype Tdouble) := 
-  cast Tdouble _ ((cast Tdouble _ ((cast Tdouble _ ((cast Tdouble _ ((cast Tdouble _ ((cast Tdouble _ (x2) * cast Tdouble _ (x5))%F64) + cast Tdouble _ ((cast Tdouble _ (x3) * cast Tdouble _ (x6))%F64))%F64) - cast Tdouble _ ((cast Tdouble _ (x2) * cast Tdouble _ (x3))%F64))%F64) - cast Tdouble _ ((cast Tdouble _ (x5) * cast Tdouble _ (x6))%F64))%F64) + cast Tdouble _ ((cast Tdouble _ (x1) * cast Tdouble _ ((cast Tdouble _ ((cast Tdouble _ ((cast Tdouble _ ((cast Tdouble _ ((cast Tdouble _ (-x1) + cast Tdouble _ (x2))%F64) + cast Tdouble _ (x3))%F64) - cast Tdouble _ (x4))%F64) + cast Tdouble _ (x5))%F64) + cast Tdouble _ (x6))%F64))%F64))%F64).
-
-Definition ex10_expr := 
- ltac:(let e' :=  HO_reify_float_expr constr:([1%positive;2%positive;3%positive;4%positive;5%positive;6%positive]) ex10 in exact e').
-
-Definition ex11_bmap_list := [Build_varinfo Tdouble 1%positive (4) (636e-2);Build_varinfo Tdouble 2%positive (4) (636e-2);Build_varinfo Tdouble 3%positive (4) (636e-2);Build_varinfo Tdouble 4%positive (4) (636e-2)].
-
-Definition ex11_bmap :=
- ltac:(let z := compute_PTree (boundsmap_of_list ex11_bmap_list) in exact z).
-
-Definition ex11_vmap_list (x1 : ftype Tdouble) (x2 : ftype Tdouble) (x3 : ftype Tdouble) (x4 : ftype Tdouble) := [(1%positive, existT ftype Tdouble x1);(2%positive, existT ftype Tdouble x2);(3%positive, existT ftype Tdouble x3);(4%positive, existT ftype Tdouble x4)].
-
-Definition ex11_vmap (x1 : ftype Tdouble) (x2 : ftype Tdouble) (x3 : ftype Tdouble) (x4 : ftype Tdouble) :=
- ltac:(let z := compute_PTree (valmap_of_list (ex11_vmap_list x1  x2  x3  x4 )) in exact z).
-
-Definition ex11 (x1 : ftype Tdouble) (x2 : ftype Tdouble) (x3 : ftype Tdouble) (x4 : ftype Tdouble) := 
-  cast Tdouble _ ((cast Tdouble _ ((cast Tdouble _ ((cast Tdouble _ ((cast Tdouble _ ((cast Tdouble _ ((cast Tdouble _ ((cast Tdouble _ ((cast Tdouble _ (x1) * cast Tdouble _ (x4))%F64) * cast Tdouble _ ((cast Tdouble _ ((cast Tdouble _ ((cast Tdouble _ (-x1) + cast Tdouble _ (x2))%F64) + cast Tdouble _ (x3))%F64) - cast Tdouble _ (x4))%F64))%F64) + cast Tdouble _ ((cast Tdouble _ (x2) * cast Tdouble _ ((cast Tdouble _ ((cast Tdouble _ ((cast Tdouble _ (x1) - cast Tdouble _ (x2))%F64) + cast Tdouble _ (x3))%F64) + cast Tdouble _ (x4))%F64))%F64))%F64) + cast Tdouble _ ((cast Tdouble _ (x3) * cast Tdouble _ ((cast Tdouble _ ((cast Tdouble _ ((cast Tdouble _ (x1) + cast Tdouble _ (x2))%F64) - cast Tdouble _ (x3))%F64) + cast Tdouble _ (x4))%F64))%F64))%F64) - cast Tdouble _ ((cast Tdouble _ ((cast Tdouble _ (x2) * cast Tdouble _ (x3))%F64) * cast Tdouble _ (x4))%F64))%F64) - cast Tdouble _ ((cast Tdouble _ (x1) * cast Tdouble _ (x3))%F64))%F64) - cast Tdouble _ ((cast Tdouble _ (x1) * cast Tdouble _ (x2))%F64))%F64) - cast Tdouble _ (x4))%F64).
-
-Definition ex11_expr := 
- ltac:(let e' :=  HO_reify_float_expr constr:([1%positive;2%positive;3%positive;4%positive]) ex11 in exact e').
-
-Definition ex12_bmap_list := [Build_varinfo Tdouble 1%positive (4) (636e-2);Build_varinfo Tdouble 2%positive (4) (636e-2);Build_varinfo Tdouble 3%positive (4) (636e-2);Build_varinfo Tdouble 4%positive (4) (636e-2);Build_varinfo Tdouble 5%positive (4) (636e-2);Build_varinfo Tdouble 6%positive (4) (636e-2)].
-
-Definition ex12_bmap :=
- ltac:(let z := compute_PTree (boundsmap_of_list ex12_bmap_list) in exact z).
-
-Definition ex12_vmap_list (x1 : ftype Tdouble) (x2 : ftype Tdouble) (x3 : ftype Tdouble) (x4 : ftype Tdouble) (x5 : ftype Tdouble) (x6 : ftype Tdouble) := [(1%positive, existT ftype Tdouble x1);(2%positive, existT ftype Tdouble x2);(3%positive, existT ftype Tdouble x3);(4%positive, existT ftype Tdouble x4);(5%positive, existT ftype Tdouble x5);(6%positive, existT ftype Tdouble x6)].
-
-Definition ex12_vmap (x1 : ftype Tdouble) (x2 : ftype Tdouble) (x3 : ftype Tdouble) (x4 : ftype Tdouble) (x5 : ftype Tdouble) (x6 : ftype Tdouble) :=
- ltac:(let z := compute_PTree (valmap_of_list (ex12_vmap_list x1  x2  x3  x4  x5  x6 )) in exact z).
-
-Definition ex12 (x1 : ftype Tdouble) (x2 : ftype Tdouble) (x3 : ftype Tdouble) (x4 : ftype Tdouble) (x5 : ftype Tdouble) (x6 : ftype Tdouble) := 
-  cast Tdouble _ ((cast Tdouble _ ((cast Tdouble _ ((cast Tdouble _ ((cast Tdouble _ ((cast Tdouble _ ((cast Tdouble _ ((cast Tdouble _ ((cast Tdouble _ (x1) * cast Tdouble _ (x4))%F64) * cast Tdouble _ ((cast Tdouble _ ((cast Tdouble _ ((cast Tdouble _ ((cast Tdouble _ ((cast Tdouble _ (-x1) + cast Tdouble _ (x2))%F64) + cast Tdouble _ (x3))%F64) - cast Tdouble _ (x4))%F64) + cast Tdouble _ (x5))%F64) + cast Tdouble _ (x6))%F64))%F64) + cast Tdouble _ ((cast Tdouble _ ((cast Tdouble _ (x2) * cast Tdouble _ (x5))%F64) * cast Tdouble _ ((cast Tdouble _ ((cast Tdouble _ ((cast Tdouble _ ((cast Tdouble _ ((cast Tdouble _ (x1) - cast Tdouble _ (x2))%F64) + cast Tdouble _ (x3))%F64) + cast Tdouble _ (x4))%F64) - cast Tdouble _ (x5))%F64) + cast Tdouble _ (x6))%F64))%F64))%F64) + cast Tdouble _ ((cast Tdouble _ ((cast Tdouble _ (x3) * cast Tdouble _ (x6))%F64) * cast Tdouble _ ((cast Tdouble _ ((cast Tdouble _ ((cast Tdouble _ ((cast Tdouble _ ((cast Tdouble _ (x1) + cast Tdouble _ (x2))%F64) - cast Tdouble _ (x3))%F64) + cast Tdouble _ (x4))%F64) + cast Tdouble _ (x5))%F64) - cast Tdouble _ (x6))%F64))%F64))%F64) - cast Tdouble _ ((cast Tdouble _ ((cast Tdouble _ (x2) * cast Tdouble _ (x3))%F64) * cast Tdouble _ (x4))%F64))%F64) - cast Tdouble _ ((cast Tdouble _ ((cast Tdouble _ (x1) * cast Tdouble _ (x3))%F64) * cast Tdouble _ (x5))%F64))%F64) - cast Tdouble _ ((cast Tdouble _ ((cast Tdouble _ (x1) * cast Tdouble _ (x2))%F64) * cast Tdouble _ (x6))%F64))%F64) - cast Tdouble _ ((cast Tdouble _ ((cast Tdouble _ (x4) * cast Tdouble _ (x5))%F64) * cast Tdouble _ (x6))%F64))%F64).
-
-Definition ex12_expr := 
- ltac:(let e' :=  HO_reify_float_expr constr:([1%positive;2%positive;3%positive;4%positive;5%positive;6%positive]) ex12 in exact e').
-
-Definition ex13_bmap_list := [Build_varinfo Tdouble 1%positive (0) (999)].
-
-Definition ex13_bmap :=
- ltac:(let z := compute_PTree (boundsmap_of_list ex13_bmap_list) in exact z).
-
-Definition ex13_vmap_list (t : ftype Tdouble) := [(1%positive, existT ftype Tdouble t)].
-
-Definition ex13_vmap (t : ftype Tdouble) :=
- ltac:(let z := compute_PTree (valmap_of_list (ex13_vmap_list t )) in exact z).
-
-Definition ex13 (t : ftype Tdouble) := 
-  cast Tdouble _ ((cast Tdouble _ (t) / cast Tdouble _ ((cast Tdouble _ (t) + cast Tdouble _ (cast Tdouble Tdouble (1)%F64))%F64))%F64).
-
-Definition ex13_expr := 
- ltac:(let e' :=  HO_reify_float_expr constr:([1%positive]) ex13 in exact e').
-
-Definition ex14_bmap_list := [Build_varinfo Tdouble 1%positive (1001e-3) (2);Build_varinfo Tdouble 2%positive (1001e-3) (2)].
-
-Definition ex14_bmap :=
- ltac:(let z := compute_PTree (boundsmap_of_list ex14_bmap_list) in exact z).
-
-Definition ex14_vmap_list (x : ftype Tdouble) (y : ftype Tdouble) := [(1%positive, existT ftype Tdouble x);(2%positive, existT ftype Tdouble y)].
-
-Definition ex14_vmap (x : ftype Tdouble) (y : ftype Tdouble) :=
- ltac:(let z := compute_PTree (valmap_of_list (ex14_vmap_list x  y )) in exact z).
-
-Definition ex14 (x : ftype Tdouble) (y : ftype Tdouble) := 
-  cast Tdouble _ (let t := (cast Tdouble _ (x) * cast Tdouble _ (y))%F64 in
-  (cast Tdouble _ ((cast Tdouble _ (t) - cast Tdouble _ (cast Tdouble Tdouble (1)%F64))%F64) / cast Tdouble _ ((cast Tdouble _ ((cast Tdouble _ (t) * cast Tdouble _ (t))%F64) - cast Tdouble _ (cast Tdouble Tdouble (1)%F64))%F64))%F64).
-
-Definition ex14_expr := 
- ltac:(let e' :=  HO_reify_float_expr constr:([1%positive;2%positive]) ex14 in exact e').
-
-Definition ex15_bmap_list := [Build_varinfo Tdouble 1%positive (0) (77617);Build_varinfo Tdouble 2%positive (0) (33096)].
-
-Definition ex15_bmap :=
- ltac:(let z := compute_PTree (boundsmap_of_list ex15_bmap_list) in exact z).
-
-Definition ex15_vmap_list (a : ftype Tdouble) (b : ftype Tdouble) := [(1%positive, existT ftype Tdouble a);(2%positive, existT ftype Tdouble b)].
-
-Definition ex15_vmap (a : ftype Tdouble) (b : ftype Tdouble) :=
- ltac:(let z := compute_PTree (valmap_of_list (ex15_vmap_list a  b )) in exact z).
-
-Definition ex15 (a : ftype Tdouble) (b : ftype Tdouble) := 
-  cast Tdouble _ (let b2 := (cast Tdouble _ (b) * cast Tdouble _ (b))%F64 in
-  let b4 := (cast Tdouble _ (b2) * cast Tdouble _ (b2))%F64 in
-  let b6 := (cast Tdouble _ (b4) * cast Tdouble _ (b2))%F64 in
-  let b8 := (cast Tdouble _ (b4) * cast Tdouble _ (b4))%F64 in
-  let a2 := (cast Tdouble _ (a) * cast Tdouble _ (a))%F64 in
-  let firstexpr := (cast Tdouble _ ((cast Tdouble _ ((cast Tdouble _ ((cast Tdouble _ ((cast Tdouble _ (cast Tdouble Tdouble (11)%F64) * cast Tdouble _ (a2))%F64) * cast Tdouble _ (b2))%F64) - cast Tdouble _ (b6))%F64) - cast Tdouble _ ((cast Tdouble _ (cast Tdouble Tdouble (121)%F64) * cast Tdouble _ (b4))%F64))%F64) - cast Tdouble _ (cast Tdouble Tdouble (2)%F64))%F64 in
-  (cast Tdouble _ ((cast Tdouble _ ((cast Tdouble _ ((cast Tdouble _ (cast Tdouble Tdouble (33375e-2)%F64) * cast Tdouble _ (b6))%F64) + cast Tdouble _ ((cast Tdouble _ (a2) * cast Tdouble _ (firstexpr))%F64))%F64) + cast Tdouble _ ((cast Tdouble _ (cast Tdouble Tdouble (55e-1)%F64) * cast Tdouble _ (b8))%F64))%F64) + cast Tdouble _ ((cast Tdouble _ (a) / cast Tdouble _ ((cast Tdouble _ (cast Tdouble Tdouble (2)%F64) * cast Tdouble _ (b))%F64))%F64))%F64).
-
-Definition ex15_expr := 
- ltac:(let e' :=  HO_reify_float_expr constr:([1%positive;2%positive]) ex15 in exact e').
-
-Definition ex16_bmap_list := [Build_varinfo Tdouble 1%positive (0) (77617);Build_varinfo Tdouble 2%positive (0) (33096)].
-
-Definition ex16_bmap :=
- ltac:(let z := compute_PTree (boundsmap_of_list ex16_bmap_list) in exact z).
-
-Definition ex16_vmap_list (a : ftype Tdouble) (b : ftype Tdouble) := [(1%positive, existT ftype Tdouble a);(2%positive, existT ftype Tdouble b)].
-
-Definition ex16_vmap (a : ftype Tdouble) (b : ftype Tdouble) :=
- ltac:(let z := compute_PTree (valmap_of_list (ex16_vmap_list a  b )) in exact z).
-
-Definition ex16 (a : ftype Tdouble) (b : ftype Tdouble) := 
-  cast Tdouble _ (let b2 := (cast Tdouble _ (b) * cast Tdouble _ (b))%F64 in
-  let b4 := (cast Tdouble _ (b2) * cast Tdouble _ (b2))%F64 in
-  let b6 := (cast Tdouble _ (b4) * cast Tdouble _ (b2))%F64 in
-  let b8 := (cast Tdouble _ (b4) * cast Tdouble _ (b4))%F64 in
-  let a2 := (cast Tdouble _ (a) * cast Tdouble _ (a))%F64 in
-  let firstexpr := (cast Tdouble _ ((cast Tdouble _ ((cast Tdouble _ ((cast Tdouble _ (cast Tdouble Tdouble (11)%F64) * cast Tdouble _ (a2))%F64) * cast Tdouble _ (b2))%F64) - cast Tdouble _ ((cast Tdouble _ (cast Tdouble Tdouble (121)%F64) * cast Tdouble _ (b4))%F64))%F64) - cast Tdouble _ (cast Tdouble Tdouble (2)%F64))%F64 in
-  (cast Tdouble _ ((cast Tdouble _ ((cast Tdouble _ ((cast Tdouble _ ((cast Tdouble _ (cast Tdouble Tdouble (33375e-2)%F64) - cast Tdouble _ (a2))%F64) * cast Tdouble _ (b6))%F64) + cast Tdouble _ ((cast Tdouble _ (a2) * cast Tdouble _ (firstexpr))%F64))%F64) + cast Tdouble _ ((cast Tdouble _ (cast Tdouble Tdouble (55e-1)%F64) * cast Tdouble _ (b8))%F64))%F64) + cast Tdouble _ ((cast Tdouble _ (a) / cast Tdouble _ ((cast Tdouble _ (cast Tdouble Tdouble (2)%F64) * cast Tdouble _ (b))%F64))%F64))%F64).
-
-Definition ex16_expr := 
- ltac:(let e' :=  HO_reify_float_expr constr:([1%positive;2%positive]) ex16 in exact e').
-
-Definition ex17_bmap_list := [Build_varinfo Tdouble 1%positive (-100) (100);Build_varinfo Tdouble 2%positive (20) (2e4);Build_varinfo Tdouble 3%positive (-30) (50)].
-
-Definition ex17_bmap :=
- ltac:(let z := compute_PTree (boundsmap_of_list ex17_bmap_list) in exact z).
-
-Definition ex17_vmap_list (u : ftype Tdouble) (v : ftype Tdouble) (t : ftype Tdouble) := [(1%positive, existT ftype Tdouble u);(2%positive, existT ftype Tdouble v);(3%positive, existT ftype Tdouble t)].
-
-Definition ex17_vmap (u : ftype Tdouble) (v : ftype Tdouble) (t : ftype Tdouble) :=
- ltac:(let z := compute_PTree (valmap_of_list (ex17_vmap_list u  v  t )) in exact z).
-
-Definition ex17 (u : ftype Tdouble) (v : ftype Tdouble) (t : ftype Tdouble) := 
-  cast Tdouble _ (let t1 := (cast Tdouble _ (cast Tdouble Tdouble (3314e-1)%F64) + cast Tdouble _ ((cast Tdouble _ (cast Tdouble Tdouble (6e-1)%F64) * cast Tdouble _ (t))%F64))%F64 in
-  (cast Tdouble _ ((cast Tdouble _ (-t1) * cast Tdouble _ (v))%F64) / cast Tdouble _ ((cast Tdouble _ ((cast Tdouble _ (t1) + cast Tdouble _ (u))%F64) * cast Tdouble _ ((cast Tdouble _ (t1) + cast Tdouble _ (u))%F64))%F64))%F64).
-
-Definition ex17_expr := 
- ltac:(let e' :=  HO_reify_float_expr constr:([1%positive;2%positive;3%positive]) ex17 in exact e').
-
-Definition ex18_bmap_list := [Build_varinfo Tdouble 1%positive (-125) (125);Build_varinfo Tdouble 2%positive (15) (25000);Build_varinfo Tdouble 3%positive (-40) (60)].
-
-Definition ex18_bmap :=
- ltac:(let z := compute_PTree (boundsmap_of_list ex18_bmap_list) in exact z).
-
-Definition ex18_vmap_list (u : ftype Tdouble) (v : ftype Tdouble) (t : ftype Tdouble) := [(1%positive, existT ftype Tdouble u);(2%positive, existT ftype Tdouble v);(3%positive, existT ftype Tdouble t)].
-
-Definition ex18_vmap (u : ftype Tdouble) (v : ftype Tdouble) (t : ftype Tdouble) :=
- ltac:(let z := compute_PTree (valmap_of_list (ex18_vmap_list u  v  t )) in exact z).
-
-Definition ex18 (u : ftype Tdouble) (v : ftype Tdouble) (t : ftype Tdouble) := 
-  cast Tdouble _ (let t1 := (cast Tdouble _ (cast Tdouble Tdouble (3314e-1)%F64) + cast Tdouble _ ((cast Tdouble _ (cast Tdouble Tdouble (6e-1)%F64) * cast Tdouble _ (t))%F64))%F64 in
-  (cast Tdouble _ ((cast Tdouble _ (-t1) * cast Tdouble _ (v))%F64) / cast Tdouble _ ((cast Tdouble _ ((cast Tdouble _ (t1) + cast Tdouble _ (u))%F64) * cast Tdouble _ ((cast Tdouble _ (t1) + cast Tdouble _ (u))%F64))%F64))%F64).
-
-Definition ex18_expr := 
- ltac:(let e' :=  HO_reify_float_expr constr:([1%positive;2%positive;3%positive]) ex18 in exact e').
-
-Definition ex19_bmap_list := [Build_varinfo Tdouble 1%positive (-30) (120);Build_varinfo Tdouble 2%positive (320) (20300);Build_varinfo Tdouble 3%positive (-50) (30)].
-
-Definition ex19_bmap :=
- ltac:(let z := compute_PTree (boundsmap_of_list ex19_bmap_list) in exact z).
-
-Definition ex19_vmap_list (u : ftype Tdouble) (v : ftype Tdouble) (t : ftype Tdouble) := [(1%positive, existT ftype Tdouble u);(2%positive, existT ftype Tdouble v);(3%positive, existT ftype Tdouble t)].
-
-Definition ex19_vmap (u : ftype Tdouble) (v : ftype Tdouble) (t : ftype Tdouble) :=
- ltac:(let z := compute_PTree (valmap_of_list (ex19_vmap_list u  v  t )) in exact z).
-
-Definition ex19 (u : ftype Tdouble) (v : ftype Tdouble) (t : ftype Tdouble) := 
-  cast Tdouble _ (let t1 := (cast Tdouble _ (cast Tdouble Tdouble (3314e-1)%F64) + cast Tdouble _ ((cast Tdouble _ (cast Tdouble Tdouble (6e-1)%F64) * cast Tdouble _ (t))%F64))%F64 in
-  (cast Tdouble _ ((cast Tdouble _ (-t1) * cast Tdouble _ (v))%F64) / cast Tdouble _ ((cast Tdouble _ ((cast Tdouble _ (t1) + cast Tdouble _ (u))%F64) * cast Tdouble _ ((cast Tdouble _ (t1) + cast Tdouble _ (u))%F64))%F64))%F64).
-
-Definition ex19_expr := 
- ltac:(let e' :=  HO_reify_float_expr constr:([1%positive;2%positive;3%positive]) ex19 in exact e').
-
-Definition ex20_bmap_list := [Build_varinfo Tdouble 1%positive (-15) (15);Build_varinfo Tdouble 2%positive (-15) (15);Build_varinfo Tdouble 3%positive (-15) (15)].
-
-Definition ex20_bmap :=
- ltac:(let z := compute_PTree (boundsmap_of_list ex20_bmap_list) in exact z).
-
-Definition ex20_vmap_list (x1 : ftype Tdouble) (x2 : ftype Tdouble) (x3 : ftype Tdouble) := [(1%positive, existT ftype Tdouble x1);(2%positive, existT ftype Tdouble x2);(3%positive, existT ftype Tdouble x3)].
-
-Definition ex20_vmap (x1 : ftype Tdouble) (x2 : ftype Tdouble) (x3 : ftype Tdouble) :=
- ltac:(let z := compute_PTree (valmap_of_list (ex20_vmap_list x1  x2  x3 )) in exact z).
-
-Definition ex20 (x1 : ftype Tdouble) (x2 : ftype Tdouble) (x3 : ftype Tdouble) := 
-  cast Tdouble _ ((cast Tdouble _ ((cast Tdouble _ ((cast Tdouble _ (-(cast Tdouble _ (x1) * cast Tdouble _ (x2))%F64) - cast Tdouble _ ((cast Tdouble _ ((cast Tdouble _ (cast Tdouble Tdouble (2)%F64) * cast Tdouble _ (x2))%F64) * cast Tdouble _ (x3))%F64))%F64) - cast Tdouble _ (x1))%F64) - cast Tdouble _ (x3))%F64).
-
-Definition ex20_expr := 
- ltac:(let e' :=  HO_reify_float_expr constr:([1%positive;2%positive;3%positive]) ex20 in exact e').
-
-Definition ex21_bmap_list := [Build_varinfo Tdouble 1%positive (-15) (15);Build_varinfo Tdouble 2%positive (-15) (15);Build_varinfo Tdouble 3%positive (-15) (15)].
-
-Definition ex21_bmap :=
- ltac:(let z := compute_PTree (boundsmap_of_list ex21_bmap_list) in exact z).
-
-Definition ex21_vmap_list (x1 : ftype Tdouble) (x2 : ftype Tdouble) (x3 : ftype Tdouble) := [(1%positive, existT ftype Tdouble x1);(2%positive, existT ftype Tdouble x2);(3%positive, existT ftype Tdouble x3)].
-
-Definition ex21_vmap (x1 : ftype Tdouble) (x2 : ftype Tdouble) (x3 : ftype Tdouble) :=
- ltac:(let z := compute_PTree (valmap_of_list (ex21_vmap_list x1  x2  x3 )) in exact z).
-
-Definition ex21 (x1 : ftype Tdouble) (x2 : ftype Tdouble) (x3 : ftype Tdouble) := 
-  cast Tdouble _ ((cast Tdouble _ ((cast Tdouble _ ((cast Tdouble _ ((cast Tdouble _ ((cast Tdouble _ ((cast Tdouble _ ((cast Tdouble _ (cast Tdouble Tdouble (2)%F64) * cast Tdouble _ (x1))%F64) * cast Tdouble _ (x2))%F64) * cast Tdouble _ (x3))%F64) + cast Tdouble _ ((cast Tdouble _ ((cast Tdouble _ (cast Tdouble Tdouble (3)%F64) * cast Tdouble _ (x3))%F64) * cast Tdouble _ (x3))%F64))%F64) - cast Tdouble _ ((cast Tdouble _ ((cast Tdouble _ ((cast Tdouble _ (x2) * cast Tdouble _ (x1))%F64) * cast Tdouble _ (x2))%F64) * cast Tdouble _ (x3))%F64))%F64) + cast Tdouble _ ((cast Tdouble _ ((cast Tdouble _ (cast Tdouble Tdouble (3)%F64) * cast Tdouble _ (x3))%F64) * cast Tdouble _ (x3))%F64))%F64) - cast Tdouble _ (x2))%F64).
-
-Definition ex21_expr := 
- ltac:(let e' :=  HO_reify_float_expr constr:([1%positive;2%positive;3%positive]) ex21 in exact e').
-
-Definition ex22_bmap_list := [Build_varinfo Tdouble 1%positive (-5) (5);Build_varinfo Tdouble 2%positive (-20) (5)].
-
-Definition ex22_bmap :=
- ltac:(let z := compute_PTree (boundsmap_of_list ex22_bmap_list) in exact z).
-
-Definition ex22_vmap_list (x1 : ftype Tdouble) (x2 : ftype Tdouble) := [(1%positive, existT ftype Tdouble x1);(2%positive, existT ftype Tdouble x2)].
-
-Definition ex22_vmap (x1 : ftype Tdouble) (x2 : ftype Tdouble) :=
- ltac:(let z := compute_PTree (valmap_of_list (ex22_vmap_list x1  x2 )) in exact z).
-
-Definition ex22 (x1 : ftype Tdouble) (x2 : ftype Tdouble) := 
-  cast Tdouble _ (let t := (cast Tdouble _ ((cast Tdouble _ ((cast Tdouble _ ((cast Tdouble _ (cast Tdouble Tdouble (3)%F64) * cast Tdouble _ (x1))%F64) * cast Tdouble _ (x1))%F64) + cast Tdouble _ ((cast Tdouble _ (cast Tdouble Tdouble (2)%F64) * cast Tdouble _ (x2))%F64))%F64) - cast Tdouble _ (x1))%F64 in
-  let t_42_ := (cast Tdouble _ ((cast Tdouble _ ((cast Tdouble _ ((cast Tdouble _ (cast Tdouble Tdouble (3)%F64) * cast Tdouble _ (x1))%F64) * cast Tdouble _ (x1))%F64) - cast Tdouble _ ((cast Tdouble _ (cast Tdouble Tdouble (2)%F64) * cast Tdouble _ (x2))%F64))%F64) - cast Tdouble _ (x1))%F64 in
-  let d := (cast Tdouble _ ((cast Tdouble _ (x1) * cast Tdouble _ (x1))%F64) + cast Tdouble _ (cast Tdouble Tdouble (1)%F64))%F64 in
-  let s := (cast Tdouble _ (t) / cast Tdouble _ (d))%F64 in
-  let s_42_ := (cast Tdouble _ (t_42_) / cast Tdouble _ (d))%F64 in
-  (cast Tdouble _ (x1) + cast Tdouble _ ((cast Tdouble _ ((cast Tdouble _ ((cast Tdouble _ ((cast Tdouble _ ((cast Tdouble _ ((cast Tdouble _ ((cast Tdouble _ ((cast Tdouble _ ((cast Tdouble _ (cast Tdouble Tdouble (2)%F64) * cast Tdouble _ (x1))%F64) * cast Tdouble _ (s))%F64) * cast Tdouble _ ((cast Tdouble _ (s) - cast Tdouble _ (cast Tdouble Tdouble (3)%F64))%F64))%F64) + cast Tdouble _ ((cast Tdouble _ ((cast Tdouble _ (x1) * cast Tdouble _ (x1))%F64) * cast Tdouble _ ((cast Tdouble _ ((cast Tdouble _ (cast Tdouble Tdouble (4)%F64) * cast Tdouble _ (s))%F64) - cast Tdouble _ (cast Tdouble Tdouble (6)%F64))%F64))%F64))%F64) * cast Tdouble _ (d))%F64) + cast Tdouble _ ((cast Tdouble _ ((cast Tdouble _ ((cast Tdouble _ (cast Tdouble Tdouble (3)%F64) * cast Tdouble _ (x1))%F64) * cast Tdouble _ (x1))%F64) * cast Tdouble _ (s))%F64))%F64) + cast Tdouble _ ((cast Tdouble _ ((cast Tdouble _ (x1) * cast Tdouble _ (x1))%F64) * cast Tdouble _ (x1))%F64))%F64) + cast Tdouble _ (x1))%F64) + cast Tdouble _ ((cast Tdouble _ (cast Tdouble Tdouble (3)%F64) * cast Tdouble _ (s_42_))%F64))%F64))%F64).
-
-Definition ex22_expr := 
- ltac:(let e' :=  HO_reify_float_expr constr:([1%positive;2%positive]) ex22 in exact e').
-
-Definition ex23_bmap_list := [Build_varinfo Tdouble 1%positive (-45e-1) (-3e-1);Build_varinfo Tdouble 2%positive (4e-1) (9e-1);Build_varinfo Tdouble 3%positive (38e-1) (78e-1)].
-
-Definition ex23_bmap :=
- ltac:(let z := compute_PTree (boundsmap_of_list ex23_bmap_list) in exact z).
-
-Definition ex23_vmap_list (v : ftype Tdouble) (w : ftype Tdouble) (r : ftype Tdouble) := [(1%positive, existT ftype Tdouble v);(2%positive, existT ftype Tdouble w);(3%positive, existT ftype Tdouble r)].
-
-Definition ex23_vmap (v : ftype Tdouble) (w : ftype Tdouble) (r : ftype Tdouble) :=
- ltac:(let z := compute_PTree (valmap_of_list (ex23_vmap_list v  w  r )) in exact z).
-
-Definition ex23 (v : ftype Tdouble) (w : ftype Tdouble) (r : ftype Tdouble) := 
-  cast Tdouble _ ((cast Tdouble _ ((cast Tdouble _ ((cast Tdouble _ (cast Tdouble Tdouble (3)%F64) + cast Tdouble _ ((cast Tdouble _ (cast Tdouble Tdouble (2)%F64) / cast Tdouble _ ((cast Tdouble _ (r) * cast Tdouble _ (r))%F64))%F64))%F64) - cast Tdouble _ ((cast Tdouble _ ((cast Tdouble _ ((cast Tdouble _ (cast Tdouble Tdouble (125e-3)%F64) * cast Tdouble _ ((cast Tdouble _ (cast Tdouble Tdouble (3)%F64) - cast Tdouble _ ((cast Tdouble _ (cast Tdouble Tdouble (2)%F64) * cast Tdouble _ (v))%F64))%F64))%F64) * cast Tdouble _ ((cast Tdouble _ ((cast Tdouble _ ((cast Tdouble _ (w) * cast Tdouble _ (w))%F64) * cast Tdouble _ (r))%F64) * cast Tdouble _ (r))%F64))%F64) / cast Tdouble _ ((cast Tdouble _ (cast Tdouble Tdouble (1)%F64) - cast Tdouble _ (v))%F64))%F64))%F64) - cast Tdouble _ (cast Tdouble Tdouble (45e-1)%F64))%F64).
-
-Definition ex23_expr := 
- ltac:(let e' :=  HO_reify_float_expr constr:([1%positive;2%positive;3%positive]) ex23 in exact e').
-
-Definition ex24_bmap_list := [Build_varinfo Tdouble 1%positive (-45e-1) (-3e-1);Build_varinfo Tdouble 2%positive (4e-1) (9e-1);Build_varinfo Tdouble 3%positive (38e-1) (78e-1)].
-
-Definition ex24_bmap :=
- ltac:(let z := compute_PTree (boundsmap_of_list ex24_bmap_list) in exact z).
-
-Definition ex24_vmap_list (v : ftype Tdouble) (w : ftype Tdouble) (r : ftype Tdouble) := [(1%positive, existT ftype Tdouble v);(2%positive, existT ftype Tdouble w);(3%positive, existT ftype Tdouble r)].
-
-Definition ex24_vmap (v : ftype Tdouble) (w : ftype Tdouble) (r : ftype Tdouble) :=
- ltac:(let z := compute_PTree (valmap_of_list (ex24_vmap_list v  w  r )) in exact z).
-
-Definition ex24 (v : ftype Tdouble) (w : ftype Tdouble) (r : ftype Tdouble) := 
-  cast Tdouble _ ((cast Tdouble _ ((cast Tdouble _ ((cast Tdouble _ (cast Tdouble Tdouble (6)%F64) * cast Tdouble _ (v))%F64) - cast Tdouble _ ((cast Tdouble _ ((cast Tdouble _ ((cast Tdouble _ (cast Tdouble Tdouble (5e-1)%F64) * cast Tdouble _ (v))%F64) * cast Tdouble _ ((cast Tdouble _ ((cast Tdouble _ ((cast Tdouble _ (w) * cast Tdouble _ (w))%F64) * cast Tdouble _ (r))%F64) * cast Tdouble _ (r))%F64))%F64) / cast Tdouble _ ((cast Tdouble _ (cast Tdouble Tdouble (1)%F64) - cast Tdouble _ (v))%F64))%F64))%F64) - cast Tdouble _ (cast Tdouble Tdouble (25e-1)%F64))%F64).
-
-Definition ex24_expr := 
- ltac:(let e' :=  HO_reify_float_expr constr:([1%positive;2%positive;3%positive]) ex24 in exact e').
-
-Definition ex25_bmap_list := [Build_varinfo Tdouble 1%positive (-45e-1) (-3e-1);Build_varinfo Tdouble 2%positive (4e-1) (9e-1);Build_varinfo Tdouble 3%positive (38e-1) (78e-1)].
-
-Definition ex25_bmap :=
- ltac:(let z := compute_PTree (boundsmap_of_list ex25_bmap_list) in exact z).
-
-Definition ex25_vmap_list (v : ftype Tdouble) (w : ftype Tdouble) (r : ftype Tdouble) := [(1%positive, existT ftype Tdouble v);(2%positive, existT ftype Tdouble w);(3%positive, existT ftype Tdouble r)].
-
-Definition ex25_vmap (v : ftype Tdouble) (w : ftype Tdouble) (r : ftype Tdouble) :=
- ltac:(let z := compute_PTree (valmap_of_list (ex25_vmap_list v  w  r )) in exact z).
-
-Definition ex25 (v : ftype Tdouble) (w : ftype Tdouble) (r : ftype Tdouble) := 
-  cast Tdouble _ ((cast Tdouble _ ((cast Tdouble _ ((cast Tdouble _ (cast Tdouble Tdouble (3)%F64) - cast Tdouble _ ((cast Tdouble _ (cast Tdouble Tdouble (2)%F64) / cast Tdouble _ ((cast Tdouble _ (r) * cast Tdouble _ (r))%F64))%F64))%F64) - cast Tdouble _ ((cast Tdouble _ ((cast Tdouble _ ((cast Tdouble _ (cast Tdouble Tdouble (125e-3)%F64) * cast Tdouble _ ((cast Tdouble _ (cast Tdouble Tdouble (1)%F64) + cast Tdouble _ ((cast Tdouble _ (cast Tdouble Tdouble (2)%F64) * cast Tdouble _ (v))%F64))%F64))%F64) * cast Tdouble _ ((cast Tdouble _ ((cast Tdouble _ ((cast Tdouble _ (w) * cast Tdouble _ (w))%F64) * cast Tdouble _ (r))%F64) * cast Tdouble _ (r))%F64))%F64) / cast Tdouble _ ((cast Tdouble _ (cast Tdouble Tdouble (1)%F64) - cast Tdouble _ (v))%F64))%F64))%F64) - cast Tdouble _ (cast Tdouble Tdouble (5e-1)%F64))%F64).
-
-Definition ex25_expr := 
- ltac:(let e' :=  HO_reify_float_expr constr:([1%positive;2%positive;3%positive]) ex25 in exact e').
-
-Definition ex26_bmap_list := [Build_varinfo Tdouble 1%positive (1e-1) (3e-1)].
-
-Definition ex26_bmap :=
- ltac:(let z := compute_PTree (boundsmap_of_list ex26_bmap_list) in exact z).
-
-Definition ex26_vmap_list (x : ftype Tdouble) := [(1%positive, existT ftype Tdouble x)].
-
-Definition ex26_vmap (x : ftype Tdouble) :=
- ltac:(let z := compute_PTree (valmap_of_list (ex26_vmap_list x )) in exact z).
-
-Definition ex26 (x : ftype Tdouble) := 
-  cast Tdouble _ (let r := cast Tdouble Tdouble (4)%F64 in
-  let k := cast Tdouble Tdouble (111e-2)%F64 in
-  (cast Tdouble _ ((cast Tdouble _ (r) * cast Tdouble _ (x))%F64) / cast Tdouble _ ((cast Tdouble _ (cast Tdouble Tdouble (1)%F64) + cast Tdouble _ ((cast Tdouble _ (x) / cast Tdouble _ (k))%F64))%F64))%F64).
-
-Definition ex26_expr := 
- ltac:(let e' :=  HO_reify_float_expr constr:([1%positive]) ex26 in exact e').
-
-Definition ex27_bmap_list := [Build_varinfo Tdouble 1%positive (1e-1) (3e-1)].
-
-Definition ex27_bmap :=
- ltac:(let z := compute_PTree (boundsmap_of_list ex27_bmap_list) in exact z).
-
-Definition ex27_vmap_list (x : ftype Tdouble) := [(1%positive, existT ftype Tdouble x)].
-
-Definition ex27_vmap (x : ftype Tdouble) :=
- ltac:(let z := compute_PTree (valmap_of_list (ex27_vmap_list x )) in exact z).
-
-Definition ex27 (x : ftype Tdouble) := 
-  cast Tdouble _ (let r := cast Tdouble Tdouble (4)%F64 in
-  let k := cast Tdouble Tdouble (111e-2)%F64 in
-  (cast Tdouble _ ((cast Tdouble _ ((cast Tdouble _ (r) * cast Tdouble _ (x))%F64) * cast Tdouble _ (x))%F64) / cast Tdouble _ ((cast Tdouble _ (cast Tdouble Tdouble (1)%F64) + cast Tdouble _ ((cast Tdouble _ ((cast Tdouble _ (x) / cast Tdouble _ (k))%F64) * cast Tdouble _ ((cast Tdouble _ (x) / cast Tdouble _ (k))%F64))%F64))%F64))%F64).
-
-Definition ex27_expr := 
- ltac:(let e' :=  HO_reify_float_expr constr:([1%positive]) ex27 in exact e').
-
-Definition ex28_bmap_list := [Build_varinfo Tdouble 1%positive (1e-1) (5e-1)].
-
-Definition ex28_bmap :=
- ltac:(let z := compute_PTree (boundsmap_of_list ex28_bmap_list) in exact z).
-
-Definition ex28_vmap_list (v : ftype Tdouble) := [(1%positive, existT ftype Tdouble v)].
-
-Definition ex28_vmap (v : ftype Tdouble) :=
- ltac:(let z := compute_PTree (valmap_of_list (ex28_vmap_list v )) in exact z).
-
-Definition ex28 (v : ftype Tdouble) := 
-  cast Tdouble _ (let p := cast Tdouble Tdouble (35e6)%F64 in
-  let a := cast Tdouble Tdouble (401e-3)%F64 in
-  let b := cast Tdouble Tdouble (427e-7)%F64 in
-  let t := cast Tdouble Tdouble (300)%F64 in
-  let n := cast Tdouble Tdouble (1000)%F64 in
-  let k := cast Tdouble Tdouble (13806503e-30)%F64 in
-  (cast Tdouble _ ((cast Tdouble _ ((cast Tdouble _ (p) + cast Tdouble _ ((cast Tdouble _ ((cast Tdouble _ (a) * cast Tdouble _ ((cast Tdouble _ (n) / cast Tdouble _ (v))%F64))%F64) * cast Tdouble _ ((cast Tdouble _ (n) / cast Tdouble _ (v))%F64))%F64))%F64) * cast Tdouble _ ((cast Tdouble _ (v) - cast Tdouble _ ((cast Tdouble _ (n) * cast Tdouble _ (b))%F64))%F64))%F64) - cast Tdouble _ ((cast Tdouble _ ((cast Tdouble _ (k) * cast Tdouble _ (n))%F64) * cast Tdouble _ (t))%F64))%F64).
-
-Definition ex28_expr := 
- ltac:(let e' :=  HO_reify_float_expr constr:([1%positive]) ex28 in exact e').
-
-Definition ex29_bmap_list := [Build_varinfo Tdouble 1%positive (0) (1)].
-
-Definition ex29_bmap :=
- ltac:(let z := compute_PTree (boundsmap_of_list ex29_bmap_list) in exact z).
-
-Definition ex29_vmap_list (x : ftype Tdouble) := [(1%positive, existT ftype Tdouble x)].
-
-Definition ex29_vmap (x : ftype Tdouble) :=
- ltac:(let z := compute_PTree (valmap_of_list (ex29_vmap_list x )) in exact z).
-
-Definition ex29 (x : ftype Tdouble) := 
-  cast Tdouble _ ((cast Tdouble _ ((cast Tdouble _ ((cast Tdouble _ ((cast Tdouble _ (cast Tdouble Tdouble (1)%F64) + cast Tdouble _ ((cast Tdouble _ (cast Tdouble Tdouble (5e-1)%F64) * cast Tdouble _ (x))%F64))%F64) - cast Tdouble _ ((cast Tdouble _ ((cast Tdouble _ (cast Tdouble Tdouble (125e-3)%F64) * cast Tdouble _ (x))%F64) * cast Tdouble _ (x))%F64))%F64) + cast Tdouble _ ((cast Tdouble _ ((cast Tdouble _ ((cast Tdouble _ (cast Tdouble Tdouble (625e-4)%F64) * cast Tdouble _ (x))%F64) * cast Tdouble _ (x))%F64) * cast Tdouble _ (x))%F64))%F64) - cast Tdouble _ ((cast Tdouble _ ((cast Tdouble _ ((cast Tdouble _ ((cast Tdouble _ (cast Tdouble Tdouble (390625e-7)%F64) * cast Tdouble _ (x))%F64) * cast Tdouble _ (x))%F64) * cast Tdouble _ (x))%F64) * cast Tdouble _ (x))%F64))%F64).
-
-Definition ex29_expr := 
- ltac:(let e' :=  HO_reify_float_expr constr:([1%positive]) ex29 in exact e').
+Definition intro_45_example_45_mixed_expr := 
+ ltac:(let e' :=  HO_reify_float_expr constr:([1%positive]) intro_45_example_45_mixed in exact e').
+
+Lemma intro_45_example_45_mixed_bound:
+	find_and_prove_roundoff_bound intro_45_example_45_mixed_bmap intro_45_example_45_mixed_expr.
+Proof.
+eexists. intro. prove_roundoff_bound.
+ -
+(*
+time "prove_rndval" prove_rndval; time "interval" interval.*)
+admit.
+-
+time "prove_roundoff_bound2" prove_roundoff_bound2;
+time "prune_terms" (prune_terms (cutoff 30)).
+time "do_interval" do_interval.
+Admitted.
+
+Definition intro_45_example_45_mixed_bound_val := Eval simpl in (proj1_sig intro_45_example_45_mixed_bound).
+Print intro_45_example_45_mixed_bound_val.
+
+Definition delta4_bmap_list := [Build_varinfo Tdouble 1%positive (4) (63504e-4);Build_varinfo Tdouble 2%positive (4) (63504e-4);Build_varinfo Tdouble 3%positive (4) (63504e-4);Build_varinfo Tdouble 4%positive (4) (63504e-4);Build_varinfo Tdouble 5%positive (4) (63504e-4);Build_varinfo Tdouble 6%positive (4) (63504e-4)].
+
+Definition delta4_bmap :=
+ ltac:(let z := compute_PTree (boundsmap_of_list delta4_bmap_list) in exact z).
+
+Definition delta4 (x1 : ftype Tdouble) (x2 : ftype Tdouble) (x3 : ftype Tdouble) (x4 : ftype Tdouble) (x5 : ftype Tdouble) (x6 : ftype Tdouble) := 
+  cast Tdouble _ ((((((((-x2) * x3)%F64 - (x1 * x4)%F64)%F64 + (x2 * x5)%F64)%F64 + (x3 * x6)%F64)%F64 - (x5 * x6)%F64)%F64 + (x1 * ((((((-x1) + x2)%F64 + x3)%F64 - x4)%F64 + x5)%F64 + x6)%F64)%F64)%F64).
+
+Definition delta4_expr := 
+ ltac:(let e' :=  HO_reify_float_expr constr:([1%positive;2%positive;3%positive;4%positive;5%positive;6%positive]) delta4 in exact e').
+
+Lemma delta4_bound:
+	find_and_prove_roundoff_bound delta4_bmap delta4_expr.
+Proof.
+eexists. intro. prove_roundoff_bound.
+ -
+time "prove_rndval" prove_rndval; time "interval" interval.
+-
+time "prove_roundoff_bound2" prove_roundoff_bound2;
+time "prune_terms" (prune_terms (cutoff 30)).
+time "do_interval" do_interval.
+Defined.
+
+Definition delta4_bound_val := Eval simpl in (proj1_sig delta4_bound).
+Print delta4_bound_val.
+
+Definition delta_bmap_list := [Build_varinfo Tdouble 1%positive (4) (63504e-4);Build_varinfo Tdouble 2%positive (4) (63504e-4);Build_varinfo Tdouble 3%positive (4) (63504e-4);Build_varinfo Tdouble 4%positive (4) (63504e-4);Build_varinfo Tdouble 5%positive (4) (63504e-4);Build_varinfo Tdouble 6%positive (4) (63504e-4)].
+
+Definition delta_bmap :=
+ ltac:(let z := compute_PTree (boundsmap_of_list delta_bmap_list) in exact z).
+
+Definition delta (x1 : ftype Tdouble) (x2 : ftype Tdouble) (x3 : ftype Tdouble) (x4 : ftype Tdouble) (x5 : ftype Tdouble) (x6 : ftype Tdouble) := 
+  cast Tdouble _ (((((((((x1 * x4)%F64 * ((((((-x1) + x2)%F64 + x3)%F64 - x4)%F64 + x5)%F64 + x6)%F64)%F64 + ((x2 * x5)%F64 * (((((x1 - x2)%F64 + x3)%F64 + x4)%F64 - x5)%F64 + x6)%F64)%F64)%F64 + ((x3 * x6)%F64 * (((((x1 + x2)%F64 - x3)%F64 + x4)%F64 + x5)%F64 - x6)%F64)%F64)%F64 + (((-x2) * x3)%F64 * x4)%F64)%F64 + (((-x1) * x3)%F64 * x5)%F64)%F64 + (((-x1) * x2)%F64 * x6)%F64)%F64 + (((-x4) * x5)%F64 * x6)%F64)%F64).
+
+Definition delta_expr := 
+ ltac:(let e' :=  HO_reify_float_expr constr:([1%positive;2%positive;3%positive;4%positive;5%positive;6%positive]) delta in exact e').
+
+Lemma delta_bound:
+	find_and_prove_roundoff_bound delta_bmap delta_expr.
+Proof.
+eexists. intro. prove_roundoff_bound.
+ -
+(*
+time "prove_rndval" prove_rndval; time "interval" interval.*)
+admit.
+-
+time "prove_roundoff_bound2" prove_roundoff_bound2;
+time "prune_terms" (prune_terms (cutoff 30)).
+time "do_interval" do_interval.
+Admitted.
+
+Definition delta_bound_val := Eval simpl in (proj1_sig delta_bound).
+Print delta_bound_val.
+
+Definition x_by_xy_bmap_list := [Build_varinfo Tsingle 1%positive (1) (4);Build_varinfo Tsingle 2%positive (1) (4)].
+
+Definition x_by_xy_bmap :=
+ ltac:(let z := compute_PTree (boundsmap_of_list x_by_xy_bmap_list) in exact z).
+
+Definition x_by_xy (x : ftype Tsingle) (y : ftype Tsingle) := 
+  cast Tsingle _ ((x / (x + y)%F32)%F32).
+
+Definition x_by_xy_expr := 
+ ltac:(let e' :=  HO_reify_float_expr constr:([1%positive;2%positive]) x_by_xy in exact e').
+
+Lemma x_by_xy_bound:
+	find_and_prove_roundoff_bound x_by_xy_bmap x_by_xy_expr.
+Proof.
+eexists. intro. prove_roundoff_bound.
+ -
+(*
+time "prove_rndval" prove_rndval; time "interval" interval.*)
+admit.
+-
+time "prove_roundoff_bound2" prove_roundoff_bound2;
+time "prune_terms" (prune_terms (cutoff 30)).
+time "do_interval" do_interval.
+Admitted.
+
+Definition x_by_xy_bound_val := Eval simpl in (proj1_sig x_by_xy_bound).
+Print x_by_xy_bound_val.
+
+Definition sum_bmap_list := [Build_varinfo Tdouble 1%positive (1) (2);Build_varinfo Tdouble 2%positive (1) (2);Build_varinfo Tdouble 3%positive (1) (2)].
+
+Definition sum_bmap :=
+ ltac:(let z := compute_PTree (boundsmap_of_list sum_bmap_list) in exact z).
+
+Definition sum (x0 : ftype Tdouble) (x1 : ftype Tdouble) (x2 : ftype Tdouble) := 
+  cast Tdouble _ (let p0 := ((x0 + x1)%F64 - x2)%F64 in
+  let p1 := ((x1 + x2)%F64 - x0)%F64 in
+  let p2 := ((x2 + x0)%F64 - x1)%F64 in
+  ((p0 + p1)%F64 + p2)%F64).
+
+Definition sum_expr := 
+ ltac:(let e' :=  HO_reify_float_expr constr:([1%positive;2%positive;3%positive]) sum in exact e').
+
+Lemma sum_bound:
+	find_and_prove_roundoff_bound sum_bmap sum_expr.
+Proof.
+eexists. intro. prove_roundoff_bound.
+ -
+time "prove_rndval" prove_rndval; time "interval" interval.
+-
+time "prove_roundoff_bound2" prove_roundoff_bound2;
+time "prune_terms" (prune_terms (cutoff 30)).
+time "do_interval" do_interval.
+Defined.
+
+Definition sum_bound_val := Eval simpl in (proj1_sig sum_bound).
+Print sum_bound_val.
+
+Definition nonlin1_bmap_list := [Build_varinfo Tdouble 1%positive (0) (999)].
+
+Definition nonlin1_bmap :=
+ ltac:(let z := compute_PTree (boundsmap_of_list nonlin1_bmap_list) in exact z).
+
+Definition nonlin1 (z : ftype Tdouble) := 
+  cast Tdouble _ ((z / (z + (1)%F64)%F64)%F64).
+
+Definition nonlin1_expr := 
+ ltac:(let e' :=  HO_reify_float_expr constr:([1%positive]) nonlin1 in exact e').
+
+Lemma nonlin1_bound:
+	find_and_prove_roundoff_bound nonlin1_bmap nonlin1_expr.
+Proof.
+eexists. intro. prove_roundoff_bound.
+ -
+(*
+time "prove_rndval" prove_rndval; time "interval" interval.*)
+admit.
+-
+time "prove_roundoff_bound2" prove_roundoff_bound2;
+time "prune_terms" (prune_terms (cutoff 30)).
+time "do_interval" do_interval.
+Admitted.
+
+Definition nonlin1_bound_val := Eval simpl in (proj1_sig nonlin1_bound).
+Print nonlin1_bound_val.
+
+Definition nonlin2_bmap_list := [Build_varinfo Tdouble 1%positive (1001e-3) (2);Build_varinfo Tdouble 2%positive (1001e-3) (2)].
+
+Definition nonlin2_bmap :=
+ ltac:(let z := compute_PTree (boundsmap_of_list nonlin2_bmap_list) in exact z).
+
+Definition nonlin2 (x : ftype Tdouble) (y : ftype Tdouble) := 
+  cast Tdouble _ (let t := (x * y)%F64 in
+  ((t - (1)%F64)%F64 / ((t * t)%F64 - (1)%F64)%F64)%F64).
+
+Definition nonlin2_expr := 
+ ltac:(let e' :=  HO_reify_float_expr constr:([1%positive;2%positive]) nonlin2 in exact e').
+
+Lemma nonlin2_bound:
+	find_and_prove_roundoff_bound nonlin2_bmap nonlin2_expr.
+Proof.
+eexists. intro. prove_roundoff_bound.
+ -
+(*
+time "prove_rndval" prove_rndval; time "interval" interval.*)
+admit.
+-
+time "prove_roundoff_bound2" prove_roundoff_bound2;
+time "prune_terms" (prune_terms (cutoff 30)).
+time "do_interval" do_interval.
+Admitted.
+
+Definition nonlin2_bound_val := Eval simpl in (proj1_sig nonlin2_bound).
+Print nonlin2_bound_val.
+
+Definition himmilbeau_bmap_list := [Build_varinfo Tdouble 1%positive (-5) (5);Build_varinfo Tdouble 2%positive (-5) (5)].
+
+Definition himmilbeau_bmap :=
+ ltac:(let z := compute_PTree (boundsmap_of_list himmilbeau_bmap_list) in exact z).
+
+Definition himmilbeau (x1 : ftype Tdouble) (x2 : ftype Tdouble) := 
+  cast Tdouble _ (let a := (((x1 * x1)%F64 + x2)%F64 - (11)%F64)%F64 in
+  let b := ((x1 + (x2 * x2)%F64)%F64 - (7)%F64)%F64 in
+  ((a * a)%F64 + (b * b)%F64)%F64).
+
+Definition himmilbeau_expr := 
+ ltac:(let e' :=  HO_reify_float_expr constr:([1%positive;2%positive]) himmilbeau in exact e').
+
+Lemma himmilbeau_bound:
+	find_and_prove_roundoff_bound himmilbeau_bmap himmilbeau_expr.
+Proof.
+eexists. intro. prove_roundoff_bound.
+ -
+time "prove_rndval" prove_rndval; time "interval" interval.
+-
+time "prove_roundoff_bound2" prove_roundoff_bound2;
+time "prune_terms" (prune_terms (cutoff 30)).
+time "do_interval" do_interval.
+Defined.
+
+Definition himmilbeau_bound_val := Eval simpl in (proj1_sig himmilbeau_bound).
+Print himmilbeau_bound_val.
+
+Definition kepler0_bmap_list := [Build_varinfo Tdouble 1%positive (4) (636e-2);Build_varinfo Tdouble 2%positive (4) (636e-2);Build_varinfo Tdouble 3%positive (4) (636e-2);Build_varinfo Tdouble 4%positive (4) (636e-2);Build_varinfo Tdouble 5%positive (4) (636e-2);Build_varinfo Tdouble 6%positive (4) (636e-2)].
+
+Definition kepler0_bmap :=
+ ltac:(let z := compute_PTree (boundsmap_of_list kepler0_bmap_list) in exact z).
+
+Definition kepler0 (x1 : ftype Tdouble) (x2 : ftype Tdouble) (x3 : ftype Tdouble) (x4 : ftype Tdouble) (x5 : ftype Tdouble) (x6 : ftype Tdouble) := 
+  cast Tdouble _ ((((((x2 * x5)%F64 + (x3 * x6)%F64)%F64 - (x2 * x3)%F64)%F64 - (x5 * x6)%F64)%F64 + (x1 * ((((((-x1) + x2)%F64 + x3)%F64 - x4)%F64 + x5)%F64 + x6)%F64)%F64)%F64).
+
+Definition kepler0_expr := 
+ ltac:(let e' :=  HO_reify_float_expr constr:([1%positive;2%positive;3%positive;4%positive;5%positive;6%positive]) kepler0 in exact e').
+
+Lemma kepler0_bound:
+	find_and_prove_roundoff_bound kepler0_bmap kepler0_expr.
+Proof.
+eexists. intro. prove_roundoff_bound.
+ -
+time "prove_rndval" prove_rndval; time "interval" interval.
+-
+time "prove_roundoff_bound2" prove_roundoff_bound2;
+time "prune_terms" (prune_terms (cutoff 30)).
+time "do_interval" do_interval.
+Defined.
+
+Definition kepler0_bound_val := Eval simpl in (proj1_sig kepler0_bound).
+Print kepler0_bound_val.
+
+Definition kepler1_bmap_list := [Build_varinfo Tdouble 1%positive (4) (636e-2);Build_varinfo Tdouble 2%positive (4) (636e-2);Build_varinfo Tdouble 3%positive (4) (636e-2);Build_varinfo Tdouble 4%positive (4) (636e-2)].
+
+Definition kepler1_bmap :=
+ ltac:(let z := compute_PTree (boundsmap_of_list kepler1_bmap_list) in exact z).
+
+Definition kepler1 (x1 : ftype Tdouble) (x2 : ftype Tdouble) (x3 : ftype Tdouble) (x4 : ftype Tdouble) := 
+  cast Tdouble _ (((((((((x1 * x4)%F64 * ((((-x1) + x2)%F64 + x3)%F64 - x4)%F64)%F64 + (x2 * (((x1 - x2)%F64 + x3)%F64 + x4)%F64)%F64)%F64 + (x3 * (((x1 + x2)%F64 - x3)%F64 + x4)%F64)%F64)%F64 - ((x2 * x3)%F64 * x4)%F64)%F64 - (x1 * x3)%F64)%F64 - (x1 * x2)%F64)%F64 - x4)%F64).
+
+Definition kepler1_expr := 
+ ltac:(let e' :=  HO_reify_float_expr constr:([1%positive;2%positive;3%positive;4%positive]) kepler1 in exact e').
+
+Lemma kepler1_bound:
+	find_and_prove_roundoff_bound kepler1_bmap kepler1_expr.
+Proof.
+eexists. intro. prove_roundoff_bound.
+ -
+time "prove_rndval" prove_rndval; time "interval" interval.
+-
+time "prove_roundoff_bound2" prove_roundoff_bound2;
+time "prune_terms" (prune_terms (cutoff 30)).
+time "do_interval" do_interval.
+Defined.
+
+Definition kepler1_bound_val := Eval simpl in (proj1_sig kepler1_bound).
+Print kepler1_bound_val.
+
+Definition kepler2_bmap_list := [Build_varinfo Tdouble 1%positive (4) (636e-2);Build_varinfo Tdouble 2%positive (4) (636e-2);Build_varinfo Tdouble 3%positive (4) (636e-2);Build_varinfo Tdouble 4%positive (4) (636e-2);Build_varinfo Tdouble 5%positive (4) (636e-2);Build_varinfo Tdouble 6%positive (4) (636e-2)].
+
+Definition kepler2_bmap :=
+ ltac:(let z := compute_PTree (boundsmap_of_list kepler2_bmap_list) in exact z).
+
+Definition kepler2 (x1 : ftype Tdouble) (x2 : ftype Tdouble) (x3 : ftype Tdouble) (x4 : ftype Tdouble) (x5 : ftype Tdouble) (x6 : ftype Tdouble) := 
+  cast Tdouble _ (((((((((x1 * x4)%F64 * ((((((-x1) + x2)%F64 + x3)%F64 - x4)%F64 + x5)%F64 + x6)%F64)%F64 + ((x2 * x5)%F64 * (((((x1 - x2)%F64 + x3)%F64 + x4)%F64 - x5)%F64 + x6)%F64)%F64)%F64 + ((x3 * x6)%F64 * (((((x1 + x2)%F64 - x3)%F64 + x4)%F64 + x5)%F64 - x6)%F64)%F64)%F64 - ((x2 * x3)%F64 * x4)%F64)%F64 - ((x1 * x3)%F64 * x5)%F64)%F64 - ((x1 * x2)%F64 * x6)%F64)%F64 - ((x4 * x5)%F64 * x6)%F64)%F64).
+
+Definition kepler2_expr := 
+ ltac:(let e' :=  HO_reify_float_expr constr:([1%positive;2%positive;3%positive;4%positive;5%positive;6%positive]) kepler2 in exact e').
+
+Lemma kepler2_bound:
+	find_and_prove_roundoff_bound kepler2_bmap kepler2_expr.
+Proof.
+eexists. intro. prove_roundoff_bound.
+ -
+time "prove_rndval" prove_rndval; time "interval" interval.
+-
+time "prove_roundoff_bound2" prove_roundoff_bound2;
+time "prune_terms" (prune_terms (cutoff 30)).
+time "do_interval" do_interval.
+Defined.
+
+Definition kepler2_bound_val := Eval simpl in (proj1_sig kepler2_bound).
+Print kepler2_bound_val.
+
+Definition intro_45_example_bmap_list := [Build_varinfo Tdouble 1%positive (0) (999)].
+
+Definition intro_45_example_bmap :=
+ ltac:(let z := compute_PTree (boundsmap_of_list intro_45_example_bmap_list) in exact z).
+
+Definition intro_45_example (t : ftype Tdouble) := 
+  cast Tdouble _ ((t / (t + (1)%F64)%F64)%F64).
+
+Definition intro_45_example_expr := 
+ ltac:(let e' :=  HO_reify_float_expr constr:([1%positive]) intro_45_example in exact e').
+
+Lemma intro_45_example_bound:
+	find_and_prove_roundoff_bound intro_45_example_bmap intro_45_example_expr.
+Proof.
+eexists. intro. prove_roundoff_bound.
+ -
+time "prove_rndval" prove_rndval; time "interval" interval.
+-
+time "prove_roundoff_bound2" prove_roundoff_bound2;
+time "prune_terms" (prune_terms (cutoff 30)).
+time "do_interval" do_interval.
+Defined.
+
+Definition intro_45_example_bound_val := Eval simpl in (proj1_sig intro_45_example_bound).
+Print intro_45_example_bound_val.
+
+Definition sec4_45_example_bmap_list := [Build_varinfo Tdouble 1%positive (1001e-3) (2);Build_varinfo Tdouble 2%positive (1001e-3) (2)].
+
+Definition sec4_45_example_bmap :=
+ ltac:(let z := compute_PTree (boundsmap_of_list sec4_45_example_bmap_list) in exact z).
+
+Definition sec4_45_example (x : ftype Tdouble) (y : ftype Tdouble) := 
+  cast Tdouble _ (let t := (x * y)%F64 in
+  ((t - (1)%F64)%F64 / ((t * t)%F64 - (1)%F64)%F64)%F64).
+
+Definition sec4_45_example_expr := 
+ ltac:(let e' :=  HO_reify_float_expr constr:([1%positive;2%positive]) sec4_45_example in exact e').
+
+Lemma sec4_45_example_bound:
+	find_and_prove_roundoff_bound sec4_45_example_bmap sec4_45_example_expr.
+Proof.
+eexists. intro. prove_roundoff_bound.
+ -
+time "prove_rndval" prove_rndval; time "interval" interval.
+-
+time "prove_roundoff_bound2" prove_roundoff_bound2;
+time "prune_terms" (prune_terms (cutoff 30)).
+time "do_interval" do_interval.
+Defined.
+
+Definition sec4_45_example_bound_val := Eval simpl in (proj1_sig sec4_45_example_bound).
+Print sec4_45_example_bound_val.
+
+Definition rump_39_s_32_example_44__32_from_32_c_32_program_bmap_list := [Build_varinfo Tdouble 1%positive (0) (77617);Build_varinfo Tdouble 2%positive (0) (33096)].
+
+Definition rump_39_s_32_example_44__32_from_32_c_32_program_bmap :=
+ ltac:(let z := compute_PTree (boundsmap_of_list rump_39_s_32_example_44__32_from_32_c_32_program_bmap_list) in exact z).
+
+Definition rump_39_s_32_example_44__32_from_32_c_32_program (a : ftype Tdouble) (b : ftype Tdouble) := 
+  cast Tdouble _ (let b2 := (b * b)%F64 in
+  let b4 := (b2 * b2)%F64 in
+  let b6 := (b4 * b2)%F64 in
+  let b8 := (b4 * b4)%F64 in
+  let a2 := (a * a)%F64 in
+  let firstexpr := ((((((11)%F64 * a2)%F64 * b2)%F64 - b6)%F64 - ((121)%F64 * b4)%F64)%F64 - (2)%F64)%F64 in
+  (((((33375e-2)%F64 * b6)%F64 + (a2 * firstexpr)%F64)%F64 + ((55e-1)%F64 * b8)%F64)%F64 + (a / ((2)%F64 * b)%F64)%F64)%F64).
+
+Definition rump_39_s_32_example_44__32_from_32_c_32_program_expr := 
+ ltac:(let e' :=  HO_reify_float_expr constr:([1%positive;2%positive]) rump_39_s_32_example_44__32_from_32_c_32_program in exact e').
+
+Lemma rump_39_s_32_example_44__32_from_32_c_32_program_bound:
+	find_and_prove_roundoff_bound rump_39_s_32_example_44__32_from_32_c_32_program_bmap rump_39_s_32_example_44__32_from_32_c_32_program_expr.
+Proof.
+eexists. intro. prove_roundoff_bound.
+ -
+time "prove_rndval" prove_rndval; time "interval" interval.
+-
+time "prove_roundoff_bound2" prove_roundoff_bound2;
+time "prune_terms" (prune_terms (cutoff 30)).
+time "do_interval" do_interval.
+Defined.
+
+Definition rump_39_s_32_example_44__32_from_32_c_32_program_bound_val := Eval simpl in (proj1_sig rump_39_s_32_example_44__32_from_32_c_32_program_bound).
+Print rump_39_s_32_example_44__32_from_32_c_32_program_bound_val.
+
+Definition rump_39_s_32_example_32_revisited_32_for_32_floating_32_point_bmap_list := [Build_varinfo Tdouble 1%positive (0) (77617);Build_varinfo Tdouble 2%positive (0) (33096)].
+
+Definition rump_39_s_32_example_32_revisited_32_for_32_floating_32_point_bmap :=
+ ltac:(let z := compute_PTree (boundsmap_of_list rump_39_s_32_example_32_revisited_32_for_32_floating_32_point_bmap_list) in exact z).
+
+Definition rump_39_s_32_example_32_revisited_32_for_32_floating_32_point (a : ftype Tdouble) (b : ftype Tdouble) := 
+  cast Tdouble _ (let b2 := (b * b)%F64 in
+  let b4 := (b2 * b2)%F64 in
+  let b6 := (b4 * b2)%F64 in
+  let b8 := (b4 * b4)%F64 in
+  let a2 := (a * a)%F64 in
+  let firstexpr := (((((11)%F64 * a2)%F64 * b2)%F64 - ((121)%F64 * b4)%F64)%F64 - (2)%F64)%F64 in
+  ((((((33375e-2)%F64 - a2)%F64 * b6)%F64 + (a2 * firstexpr)%F64)%F64 + ((55e-1)%F64 * b8)%F64)%F64 + (a / ((2)%F64 * b)%F64)%F64)%F64).
+
+Definition rump_39_s_32_example_32_revisited_32_for_32_floating_32_point_expr := 
+ ltac:(let e' :=  HO_reify_float_expr constr:([1%positive;2%positive]) rump_39_s_32_example_32_revisited_32_for_32_floating_32_point in exact e').
+
+Lemma rump_39_s_32_example_32_revisited_32_for_32_floating_32_point_bound:
+	find_and_prove_roundoff_bound rump_39_s_32_example_32_revisited_32_for_32_floating_32_point_bmap rump_39_s_32_example_32_revisited_32_for_32_floating_32_point_expr.
+Proof.
+eexists. intro. prove_roundoff_bound.
+ -
+time "prove_rndval" prove_rndval; time "interval" interval.
+-
+time "prove_roundoff_bound2" prove_roundoff_bound2;
+time "prune_terms" (prune_terms (cutoff 30)).
+time "do_interval" do_interval.
+Defined.
+
+Definition rump_39_s_32_example_32_revisited_32_for_32_floating_32_point_bound_val := Eval simpl in (proj1_sig rump_39_s_32_example_32_revisited_32_for_32_floating_32_point_bound).
+Print rump_39_s_32_example_32_revisited_32_for_32_floating_32_point_bound_val.
+
+Definition doppler1_bmap_list := [Build_varinfo Tdouble 1%positive (-100) (100);Build_varinfo Tdouble 2%positive (20) (2e4);Build_varinfo Tdouble 3%positive (-30) (50)].
+
+Definition doppler1_bmap :=
+ ltac:(let z := compute_PTree (boundsmap_of_list doppler1_bmap_list) in exact z).
+
+Definition doppler1 (u : ftype Tdouble) (v : ftype Tdouble) (t : ftype Tdouble) := 
+  cast Tdouble _ (let t1 := ((3314e-1)%F64 + ((6e-1)%F64 * t)%F64)%F64 in
+  (((-t1) * v)%F64 / ((t1 + u)%F64 * (t1 + u)%F64)%F64)%F64).
+
+Definition doppler1_expr := 
+ ltac:(let e' :=  HO_reify_float_expr constr:([1%positive;2%positive;3%positive]) doppler1 in exact e').
+
+Lemma doppler1_bound:
+	find_and_prove_roundoff_bound doppler1_bmap doppler1_expr.
+Proof.
+eexists. intro. prove_roundoff_bound.
+ -
+time "prove_rndval" prove_rndval; time "interval" interval.
+-
+time "prove_roundoff_bound2" prove_roundoff_bound2;
+time "prune_terms" (prune_terms (cutoff 30)).
+time "do_interval" do_interval.
+Defined.
+
+Definition doppler1_bound_val := Eval simpl in (proj1_sig doppler1_bound).
+Print doppler1_bound_val.
+
+Definition doppler2_bmap_list := [Build_varinfo Tdouble 1%positive (-125) (125);Build_varinfo Tdouble 2%positive (15) (25000);Build_varinfo Tdouble 3%positive (-40) (60)].
+
+Definition doppler2_bmap :=
+ ltac:(let z := compute_PTree (boundsmap_of_list doppler2_bmap_list) in exact z).
+
+Definition doppler2 (u : ftype Tdouble) (v : ftype Tdouble) (t : ftype Tdouble) := 
+  cast Tdouble _ (let t1 := ((3314e-1)%F64 + ((6e-1)%F64 * t)%F64)%F64 in
+  (((-t1) * v)%F64 / ((t1 + u)%F64 * (t1 + u)%F64)%F64)%F64).
+
+Definition doppler2_expr := 
+ ltac:(let e' :=  HO_reify_float_expr constr:([1%positive;2%positive;3%positive]) doppler2 in exact e').
+
+Lemma doppler2_bound:
+	find_and_prove_roundoff_bound doppler2_bmap doppler2_expr.
+Proof.
+eexists. intro. prove_roundoff_bound.
+ -
+time "prove_rndval" prove_rndval; time "interval" interval.
+-
+time "prove_roundoff_bound2" prove_roundoff_bound2;
+time "prune_terms" (prune_terms (cutoff 30)).
+time "do_interval" do_interval.
+Defined.
+
+Definition doppler2_bound_val := Eval simpl in (proj1_sig doppler2_bound).
+Print doppler2_bound_val.
+
+Definition doppler3_bmap_list := [Build_varinfo Tdouble 1%positive (-30) (120);Build_varinfo Tdouble 2%positive (320) (20300);Build_varinfo Tdouble 3%positive (-50) (30)].
+
+Definition doppler3_bmap :=
+ ltac:(let z := compute_PTree (boundsmap_of_list doppler3_bmap_list) in exact z).
+
+Definition doppler3 (u : ftype Tdouble) (v : ftype Tdouble) (t : ftype Tdouble) := 
+  cast Tdouble _ (let t1 := ((3314e-1)%F64 + ((6e-1)%F64 * t)%F64)%F64 in
+  (((-t1) * v)%F64 / ((t1 + u)%F64 * (t1 + u)%F64)%F64)%F64).
+
+Definition doppler3_expr := 
+ ltac:(let e' :=  HO_reify_float_expr constr:([1%positive;2%positive;3%positive]) doppler3 in exact e').
+
+Lemma doppler3_bound:
+	find_and_prove_roundoff_bound doppler3_bmap doppler3_expr.
+Proof.
+eexists. intro. prove_roundoff_bound.
+ -
+time "prove_rndval" prove_rndval; time "interval" interval.
+-
+time "prove_roundoff_bound2" prove_roundoff_bound2;
+time "prune_terms" (prune_terms (cutoff 30)).
+time "do_interval" do_interval.
+Defined.
+
+Definition doppler3_bound_val := Eval simpl in (proj1_sig doppler3_bound).
+Print doppler3_bound_val.
+
+Definition rigidbody1_bmap_list := [Build_varinfo Tdouble 1%positive (-15) (15);Build_varinfo Tdouble 2%positive (-15) (15);Build_varinfo Tdouble 3%positive (-15) (15)].
+
+Definition rigidbody1_bmap :=
+ ltac:(let z := compute_PTree (boundsmap_of_list rigidbody1_bmap_list) in exact z).
+
+Definition rigidbody1 (x1 : ftype Tdouble) (x2 : ftype Tdouble) (x3 : ftype Tdouble) := 
+  cast Tdouble _ (((((-(x1 * x2)%F64) - (((2)%F64 * x2)%F64 * x3)%F64)%F64 - x1)%F64 - x3)%F64).
+
+Definition rigidbody1_expr := 
+ ltac:(let e' :=  HO_reify_float_expr constr:([1%positive;2%positive;3%positive]) rigidbody1 in exact e').
+
+Lemma rigidbody1_bound:
+	find_and_prove_roundoff_bound rigidbody1_bmap rigidbody1_expr.
+Proof.
+eexists. intro. prove_roundoff_bound.
+ -
+time "prove_rndval" prove_rndval; time "interval" interval.
+-
+time "prove_roundoff_bound2" prove_roundoff_bound2;
+time "prune_terms" (prune_terms (cutoff 30)).
+time "do_interval" do_interval.
+Defined.
+
+Definition rigidbody1_bound_val := Eval simpl in (proj1_sig rigidbody1_bound).
+Print rigidbody1_bound_val.
+
+Definition rigidbody2_bmap_list := [Build_varinfo Tdouble 1%positive (-15) (15);Build_varinfo Tdouble 2%positive (-15) (15);Build_varinfo Tdouble 3%positive (-15) (15)].
+
+Definition rigidbody2_bmap :=
+ ltac:(let z := compute_PTree (boundsmap_of_list rigidbody2_bmap_list) in exact z).
+
+Definition rigidbody2 (x1 : ftype Tdouble) (x2 : ftype Tdouble) (x3 : ftype Tdouble) := 
+  cast Tdouble _ (((((((((2)%F64 * x1)%F64 * x2)%F64 * x3)%F64 + (((3)%F64 * x3)%F64 * x3)%F64)%F64 - (((x2 * x1)%F64 * x2)%F64 * x3)%F64)%F64 + (((3)%F64 * x3)%F64 * x3)%F64)%F64 - x2)%F64).
+
+Definition rigidbody2_expr := 
+ ltac:(let e' :=  HO_reify_float_expr constr:([1%positive;2%positive;3%positive]) rigidbody2 in exact e').
+
+Lemma rigidbody2_bound:
+	find_and_prove_roundoff_bound rigidbody2_bmap rigidbody2_expr.
+Proof.
+eexists. intro. prove_roundoff_bound.
+ -
+time "prove_rndval" prove_rndval; time "interval" interval.
+-
+time "prove_roundoff_bound2" prove_roundoff_bound2;
+time "prune_terms" (prune_terms (cutoff 30)).
+time "do_interval" do_interval.
+Defined.
+
+Definition rigidbody2_bound_val := Eval simpl in (proj1_sig rigidbody2_bound).
+Print rigidbody2_bound_val.
+
+Definition jetengine_bmap_list := [Build_varinfo Tdouble 1%positive (-5) (5);Build_varinfo Tdouble 2%positive (-20) (5)].
+
+Definition jetengine_bmap :=
+ ltac:(let z := compute_PTree (boundsmap_of_list jetengine_bmap_list) in exact z).
+
+Definition jetengine (x1 : ftype Tdouble) (x2 : ftype Tdouble) := 
+  cast Tdouble _ (let t := (((((3)%F64 * x1)%F64 * x1)%F64 + ((2)%F64 * x2)%F64)%F64 - x1)%F64 in
+  let t_42_ := (((((3)%F64 * x1)%F64 * x1)%F64 - ((2)%F64 * x2)%F64)%F64 - x1)%F64 in
+  let d := ((x1 * x1)%F64 + (1)%F64)%F64 in
+  let s := (t / d)%F64 in
+  let s_42_ := (t_42_ / d)%F64 in
+  (x1 + ((((((((((2)%F64 * x1)%F64 * s)%F64 * (s - (3)%F64)%F64)%F64 + ((x1 * x1)%F64 * (((4)%F64 * s)%F64 - (6)%F64)%F64)%F64)%F64 * d)%F64 + ((((3)%F64 * x1)%F64 * x1)%F64 * s)%F64)%F64 + ((x1 * x1)%F64 * x1)%F64)%F64 + x1)%F64 + ((3)%F64 * s_42_)%F64)%F64)%F64).
+
+Definition jetengine_expr := 
+ ltac:(let e' :=  HO_reify_float_expr constr:([1%positive;2%positive]) jetengine in exact e').
+
+Lemma jetengine_bound:
+	find_and_prove_roundoff_bound jetengine_bmap jetengine_expr.
+Proof.
+eexists. intro. prove_roundoff_bound.
+ -
+time "prove_rndval" prove_rndval; time "interval" interval.
+-
+time "prove_roundoff_bound2" prove_roundoff_bound2;
+time "prune_terms" (prune_terms (cutoff 30)).
+time "do_interval" do_interval.
+Defined.
+
+Definition jetengine_bound_val := Eval simpl in (proj1_sig jetengine_bound).
+Print jetengine_bound_val.
+
+Definition turbine1_bmap_list := [Build_varinfo Tdouble 1%positive (-45e-1) (-3e-1);Build_varinfo Tdouble 2%positive (4e-1) (9e-1);Build_varinfo Tdouble 3%positive (38e-1) (78e-1)].
+
+Definition turbine1_bmap :=
+ ltac:(let z := compute_PTree (boundsmap_of_list turbine1_bmap_list) in exact z).
+
+Definition turbine1 (v : ftype Tdouble) (w : ftype Tdouble) (r : ftype Tdouble) := 
+  cast Tdouble _ (((((3)%F64 + ((2)%F64 / (r * r)%F64)%F64)%F64 - ((((125e-3)%F64 * ((3)%F64 - ((2)%F64 * v)%F64)%F64)%F64 * (((w * w)%F64 * r)%F64 * r)%F64)%F64 / ((1)%F64 - v)%F64)%F64)%F64 - (45e-1)%F64)%F64).
+
+Definition turbine1_expr := 
+ ltac:(let e' :=  HO_reify_float_expr constr:([1%positive;2%positive;3%positive]) turbine1 in exact e').
+
+Lemma turbine1_bound:
+	find_and_prove_roundoff_bound turbine1_bmap turbine1_expr.
+Proof.
+eexists. intro. prove_roundoff_bound.
+ -
+time "prove_rndval" prove_rndval; time "interval" interval.
+-
+time "prove_roundoff_bound2" prove_roundoff_bound2;
+time "prune_terms" (prune_terms (cutoff 30)).
+time "do_interval" do_interval.
+Defined.
+
+Definition turbine1_bound_val := Eval simpl in (proj1_sig turbine1_bound).
+Print turbine1_bound_val.
+
+Definition turbine2_bmap_list := [Build_varinfo Tdouble 1%positive (-45e-1) (-3e-1);Build_varinfo Tdouble 2%positive (4e-1) (9e-1);Build_varinfo Tdouble 3%positive (38e-1) (78e-1)].
+
+Definition turbine2_bmap :=
+ ltac:(let z := compute_PTree (boundsmap_of_list turbine2_bmap_list) in exact z).
+
+Definition turbine2 (v : ftype Tdouble) (w : ftype Tdouble) (r : ftype Tdouble) := 
+  cast Tdouble _ (((((6)%F64 * v)%F64 - ((((5e-1)%F64 * v)%F64 * (((w * w)%F64 * r)%F64 * r)%F64)%F64 / ((1)%F64 - v)%F64)%F64)%F64 - (25e-1)%F64)%F64).
+
+Definition turbine2_expr := 
+ ltac:(let e' :=  HO_reify_float_expr constr:([1%positive;2%positive;3%positive]) turbine2 in exact e').
+
+Lemma turbine2_bound:
+	find_and_prove_roundoff_bound turbine2_bmap turbine2_expr.
+Proof.
+eexists. intro. prove_roundoff_bound.
+ -
+time "prove_rndval" prove_rndval; time "interval" interval.
+-
+time "prove_roundoff_bound2" prove_roundoff_bound2;
+time "prune_terms" (prune_terms (cutoff 30)).
+time "do_interval" do_interval.
+Defined.
+
+Definition turbine2_bound_val := Eval simpl in (proj1_sig turbine2_bound).
+Print turbine2_bound_val.
+
+Definition turbine3_bmap_list := [Build_varinfo Tdouble 1%positive (-45e-1) (-3e-1);Build_varinfo Tdouble 2%positive (4e-1) (9e-1);Build_varinfo Tdouble 3%positive (38e-1) (78e-1)].
+
+Definition turbine3_bmap :=
+ ltac:(let z := compute_PTree (boundsmap_of_list turbine3_bmap_list) in exact z).
+
+Definition turbine3 (v : ftype Tdouble) (w : ftype Tdouble) (r : ftype Tdouble) := 
+  cast Tdouble _ (((((3)%F64 - ((2)%F64 / (r * r)%F64)%F64)%F64 - ((((125e-3)%F64 * ((1)%F64 + ((2)%F64 * v)%F64)%F64)%F64 * (((w * w)%F64 * r)%F64 * r)%F64)%F64 / ((1)%F64 - v)%F64)%F64)%F64 - (5e-1)%F64)%F64).
+
+Definition turbine3_expr := 
+ ltac:(let e' :=  HO_reify_float_expr constr:([1%positive;2%positive;3%positive]) turbine3 in exact e').
+
+Lemma turbine3_bound:
+	find_and_prove_roundoff_bound turbine3_bmap turbine3_expr.
+Proof.
+eexists. intro. prove_roundoff_bound.
+ -
+time "prove_rndval" prove_rndval; time "interval" interval.
+-
+time "prove_roundoff_bound2" prove_roundoff_bound2;
+time "prune_terms" (prune_terms (cutoff 30)).
+time "do_interval" do_interval.
+Defined.
+
+Definition turbine3_bound_val := Eval simpl in (proj1_sig turbine3_bound).
+Print turbine3_bound_val.
+
+Definition verhulst_bmap_list := [Build_varinfo Tdouble 1%positive (1e-1) (3e-1)].
+
+Definition verhulst_bmap :=
+ ltac:(let z := compute_PTree (boundsmap_of_list verhulst_bmap_list) in exact z).
+
+Definition verhulst (x : ftype Tdouble) := 
+  cast Tdouble _ (let r := (4)%F64 in
+  let k := (111e-2)%F64 in
+  ((r * x)%F64 / ((1)%F64 + (x / k)%F64)%F64)%F64).
+
+Definition verhulst_expr := 
+ ltac:(let e' :=  HO_reify_float_expr constr:([1%positive]) verhulst in exact e').
+
+Lemma verhulst_bound:
+	find_and_prove_roundoff_bound verhulst_bmap verhulst_expr.
+Proof.
+eexists. intro. prove_roundoff_bound.
+ -
+time "prove_rndval" prove_rndval; time "interval" interval.
+-
+time "prove_roundoff_bound2" prove_roundoff_bound2;
+time "prune_terms" (prune_terms (cutoff 30)).
+time "do_interval" do_interval.
+Defined.
+
+Definition verhulst_bound_val := Eval simpl in (proj1_sig verhulst_bound).
+Print verhulst_bound_val.
+
+Definition predatorprey_bmap_list := [Build_varinfo Tdouble 1%positive (1e-1) (3e-1)].
+
+Definition predatorprey_bmap :=
+ ltac:(let z := compute_PTree (boundsmap_of_list predatorprey_bmap_list) in exact z).
+
+Definition predatorprey (x : ftype Tdouble) := 
+  cast Tdouble _ (let r := (4)%F64 in
+  let k := (111e-2)%F64 in
+  (((r * x)%F64 * x)%F64 / ((1)%F64 + ((x / k)%F64 * (x / k)%F64)%F64)%F64)%F64).
+
+Definition predatorprey_expr := 
+ ltac:(let e' :=  HO_reify_float_expr constr:([1%positive]) predatorprey in exact e').
+
+Lemma predatorprey_bound:
+	find_and_prove_roundoff_bound predatorprey_bmap predatorprey_expr.
+Proof.
+eexists. intro. prove_roundoff_bound.
+ -
+time "prove_rndval" prove_rndval; time "interval" interval.
+-
+time "prove_roundoff_bound2" prove_roundoff_bound2;
+time "prune_terms" (prune_terms (cutoff 30)).
+time "do_interval" do_interval.
+Defined.
+
+Definition predatorprey_bound_val := Eval simpl in (proj1_sig predatorprey_bound).
+Print predatorprey_bound_val.
+
+Definition carbongas_bmap_list := [Build_varinfo Tdouble 1%positive (1e-1) (5e-1)].
+
+Definition carbongas_bmap :=
+ ltac:(let z := compute_PTree (boundsmap_of_list carbongas_bmap_list) in exact z).
+
+Definition carbongas (v : ftype Tdouble) := 
+  cast Tdouble _ (let p := (35e6)%F64 in
+  let a := (401e-3)%F64 in
+  let b := (427e-7)%F64 in
+  let t := (300)%F64 in
+  let n := (1000)%F64 in
+  let k := (13806503e-30)%F64 in
+  (((p + ((a * (n / v)%F64)%F64 * (n / v)%F64)%F64)%F64 * (v - (n * b)%F64)%F64)%F64 - ((k * n)%F64 * t)%F64)%F64).
+
+Definition carbongas_expr := 
+ ltac:(let e' :=  HO_reify_float_expr constr:([1%positive]) carbongas in exact e').
+
+Lemma carbongas_bound:
+	find_and_prove_roundoff_bound carbongas_bmap carbongas_expr.
+Proof.
+eexists. intro. prove_roundoff_bound.
+ -
+time "prove_rndval" prove_rndval; time "interval" interval.
+-
+time "prove_roundoff_bound2" prove_roundoff_bound2;
+time "prune_terms" (prune_terms (cutoff 30)).
+time "do_interval" do_interval.
+Defined.
+
+Definition carbongas_bound_val := Eval simpl in (proj1_sig carbongas_bound).
+Print carbongas_bound_val.
+
+Definition sqroot_bmap_list := [Build_varinfo Tdouble 1%positive (0) (1)].
+
+Definition sqroot_bmap :=
+ ltac:(let z := compute_PTree (boundsmap_of_list sqroot_bmap_list) in exact z).
+
+Definition sqroot (x : ftype Tdouble) := 
+  cast Tdouble _ ((((((1)%F64 + ((5e-1)%F64 * x)%F64)%F64 - (((125e-3)%F64 * x)%F64 * x)%F64)%F64 + ((((625e-4)%F64 * x)%F64 * x)%F64 * x)%F64)%F64 - (((((390625e-7)%F64 * x)%F64 * x)%F64 * x)%F64 * x)%F64)%F64).
+
+Definition sqroot_expr := 
+ ltac:(let e' :=  HO_reify_float_expr constr:([1%positive]) sqroot in exact e').
+
+Lemma sqroot_bound:
+	find_and_prove_roundoff_bound sqroot_bmap sqroot_expr.
+Proof.
+eexists. intro. prove_roundoff_bound.
+ -
+time "prove_rndval" prove_rndval; time "interval" interval.
+-
+time "prove_roundoff_bound2" prove_roundoff_bound2;
+time "prune_terms" (prune_terms (cutoff 30)).
+time "do_interval" do_interval.
+Defined.
+
+Definition sqroot_bound_val := Eval simpl in (proj1_sig sqroot_bound).
+Print sqroot_bound_val.
 
 End WITHNANS.
+Close R_scope.
